Solved: all unproven lemmas with [sm_valid] and [loc_alloc].

compcomp/InliningproofEFF.v
@@ -25,55 +25,228 @@ Require Import effect_simulations_lemmas.
 
 
 Require Export Axioms.
-(*Require Import CminorSel_coop.*)
 Require Import RTL_eff.
 Require Import RTL_coop.
-
-Check sepcomp.effect_simulations_lemmas.inj_simulation_star.
 
 Load Santiago_tactics.
 
 Variable SrcProg: RTL.program.
 Variable TrgProg: RTL.program.
 Hypothesis TRANSF: transf_program SrcProg = OK TrgProg.
-Let SrcGe : RTL.genv := Genv.globalenv SrcProg.
-Let TrgGe : RTL.genv := Genv.globalenv TrgProg.
+Let ge : RTL.genv := Genv.globalenv SrcProg.
+Let tge : RTL.genv := Genv.globalenv TrgProg.
 Let fenv := funenv_program SrcProg.
 
-
-Lemma function_ptr_translated:
-  forall (b: block) (f: fundef),
-  Genv.find_funct_ptr SrcGe b = Some f ->
-  exists f', Genv.find_funct_ptr TrgGe b = Some f' /\ Inlining.transf_fundef fenv f = OK f'.
-Proof (Genv.find_funct_ptr_transf_partial (transf_fundef fenv) _ TRANSF).
-
 Lemma symbols_preserved:
-  forall (s: ident), Genv.find_symbol TrgGe s = Genv.find_symbol SrcGe s.
+  forall (s: ident), Genv.find_symbol tge s = Genv.find_symbol ge s.
 Proof.
   intros. apply Genv.find_symbol_transf_partial with (transf_fundef fenv). apply TRANSF.
 Qed.
 
 Lemma varinfo_preserved:
-  forall b, Genv.find_var_info TrgGe b = Genv.find_var_info SrcGe b.
+  forall b, Genv.find_var_info tge b = Genv.find_var_info ge b.
 Proof.
   intros. apply Genv.find_var_info_transf_partial with (transf_fundef fenv). apply TRANSF.
 Qed.
 
-(*LENB: GFP as in selectionproofEFF*)
-(*Definition globalfunction_ptr_inject (j:meminj):=
-  forall b f, Genv.find_funct_ptr SrcGe b = Some f -> 
-              j b = Some(b,0) /\ isGlobalBlock SrcGe b = true. *)
+Lemma functions_translated:
+  forall (v: val) (f: fundef),
+    Genv.find_funct ge v = Some f ->
+    exists f', Genv.find_funct tge v = Some f' /\ transf_fundef fenv f = OK f'.
+Proof.
+  eapply (Genv.find_funct_transf_partial (transf_fundef fenv) _ TRANSF).
+Qed.
+Lemma function_ptr_translated:
+  forall (b: block) (f: fundef),
+    Genv.find_funct_ptr ge b = Some f ->
+    exists f', Genv.find_funct_ptr tge b = Some f' /\ transf_fundef fenv f = OK f'.
+Proof.
+eapply (Genv.find_funct_ptr_transf_partial (transf_fundef fenv) _ TRANSF).
+Qed.
+Lemma sig_function_translated:
+  forall f f', transf_fundef fenv f = OK f' -> funsig f' = funsig f.
+Proof.
+  intros. destruct f; Errors.monadInv H.
+  exploit transf_function_spec; eauto. intros SP; inv SP. auto. 
+  auto.
+Qed.
 
-(*The new match_states*)
 
-(*Tool kit for match states: *)
+(** ** Properties of contexts and relocations *)
+
+Remark sreg_below_diff:
+  forall ctx r r', Plt r' ctx.(dreg) -> sreg ctx r <> r'.
+Proof.
+  intros. zify. unfold sreg; rewrite shiftpos_eq. xomega. 
+Qed.
+
+Remark context_below_diff:
+  forall ctx1 ctx2 r1 r2,
+    context_below ctx1 ctx2 -> Ple r1 ctx1.(mreg) -> sreg ctx1 r1 <> sreg ctx2 r2.
+Proof.
+  intros. red in H. zify. unfold sreg; rewrite ! shiftpos_eq. xomega.
+Qed.
+
+Remark context_below_lt:
+  forall ctx1 ctx2 r, context_below ctx1 ctx2 -> Ple r ctx1.(mreg) -> Plt (sreg ctx1 r) ctx2.(dreg).
+Proof.
+  intros. red in H. unfold Plt; zify. unfold sreg; rewrite shiftpos_eq. 
+  xomega.
+Qed.
+
+(** ** Agreement between register sets before and after inlining. *)
 
 Definition agree_regs (F: meminj) (ctx: context) (rs rs': regset) :=
   (forall r, Ple r ctx.(mreg) -> val_inject F rs#r rs'#(sreg ctx r))
-/\(forall r, Plt ctx.(mreg) r -> rs#r = Vundef).
+  /\(forall r, Plt ctx.(mreg) r -> rs#r = Vundef).
 
 Definition val_reg_charact (F: meminj) (ctx: context) (rs': regset) (v: val) (r: reg) :=
   (Plt ctx.(mreg) r /\ v = Vundef) \/ (Ple r ctx.(mreg) /\ val_inject F v rs'#(sreg ctx r)).
+
+Remark Plt_Ple_dec:
+  forall p q, {Plt p q} + {Ple q p}.
+Proof.
+  intros. destruct (plt p q). left; auto. right; xomega.
+Qed.
+
+Lemma agree_val_reg_gen:
+  forall F ctx rs rs' r, agree_regs F ctx rs rs' -> val_reg_charact F ctx rs' rs#r r.
+Proof.
+  intros. destruct H as [A B].
+  destruct (Plt_Ple_dec (mreg ctx) r). 
+  left. rewrite B; auto. 
+  right. auto.
+Qed.
+
+Lemma agree_val_regs_gen:
+  forall F ctx rs rs' rl,
+    agree_regs F ctx rs rs' -> list_forall2 (val_reg_charact F ctx rs') rs##rl rl.
+Proof.
+  induction rl; intros; constructor; auto. apply agree_val_reg_gen; auto.
+Qed.
+
+Lemma agree_val_reg:
+  forall F ctx rs rs' r, agree_regs F ctx rs rs' -> val_inject F rs#r rs'#(sreg ctx r).
+Proof.
+  intros. exploit agree_val_reg_gen; eauto. instantiate (1 := r). intros [[A B] | [A B]].
+  rewrite B; auto.
+  auto.
+Qed.
+
+Lemma agree_val_regs:
+  forall F ctx rs rs' rl, agree_regs F ctx rs rs' -> val_list_inject F rs##rl rs'##(sregs ctx rl).
+Proof.
+  induction rl; intros; simpl. constructor. constructor; auto. apply agree_val_reg; auto.
+Qed.
+
+Lemma agree_set_reg:
+  forall F ctx rs rs' r v v',
+    agree_regs F ctx rs rs' ->
+    val_inject F v v' ->
+    Ple r ctx.(mreg) ->
+    agree_regs F ctx (rs#r <- v) (rs'#(sreg ctx r) <- v').
+Proof.
+  unfold agree_regs; intros. destruct H. split; intros.
+  repeat rewrite Regmap.gsspec. 
+  destruct (peq r0 r). subst r0. rewrite peq_true. auto.
+  rewrite peq_false. auto. apply shiftpos_diff; auto. 
+  rewrite Regmap.gso. auto. xomega. 
+Qed.
+
+Lemma agree_set_reg_undef:
+  forall F ctx rs rs' r v',
+    agree_regs F ctx rs rs' ->
+    agree_regs F ctx (rs#r <- Vundef) (rs'#(sreg ctx r) <- v').
+Proof.
+  unfold agree_regs; intros. destruct H. split; intros.
+  repeat rewrite Regmap.gsspec. 
+  destruct (peq r0 r). subst r0. rewrite peq_true. auto.
+  rewrite peq_false. auto. apply shiftpos_diff; auto. 
+  rewrite Regmap.gsspec. destruct (peq r0 r); auto. 
+Qed.
+
+Lemma agree_set_reg_undef':
+  forall F ctx rs rs' r,
+    agree_regs F ctx rs rs' ->
+    agree_regs F ctx (rs#r <- Vundef) rs'.
+Proof.
+  unfold agree_regs; intros. destruct H. split; intros.
+  rewrite Regmap.gsspec. 
+  destruct (peq r0 r). subst r0. auto. auto.
+  rewrite Regmap.gsspec. destruct (peq r0 r); auto. 
+Qed.
+
+Lemma agree_regs_invariant:
+  forall F ctx rs rs1 rs2,
+    agree_regs F ctx rs rs1 ->
+    (forall r, Ple ctx.(dreg) r -> Plt r (ctx.(dreg) + ctx.(mreg)) -> rs2#r = rs1#r) ->
+    agree_regs F ctx rs rs2.
+Proof.
+  unfold agree_regs; intros. destruct H. split; intros.
+  rewrite H0. auto. 
+  apply shiftpos_above.
+  eapply Plt_le_trans. apply shiftpos_below. xomega.
+  apply H1; auto.
+Qed.
+
+Lemma agree_regs_incr:
+  forall F ctx rs1 rs2 F',
+    agree_regs F ctx rs1 rs2 ->
+    inject_incr F F' ->
+    agree_regs F' ctx rs1 rs2.
+Proof.
+  intros. destruct H. split; intros. eauto. auto. 
+Qed.
+
+Remark agree_regs_init:
+  forall F ctx rs, agree_regs F ctx (Regmap.init Vundef) rs.
+Proof.
+  intros; split; intros. rewrite Regmap.gi; auto. rewrite Regmap.gi; auto. 
+Qed.
+
+Lemma agree_regs_init_regs:
+  forall F ctx rl vl vl',
+    val_list_inject F vl vl' ->
+    (forall r, In r rl -> Ple r ctx.(mreg)) ->
+    agree_regs F ctx (init_regs vl rl) (init_regs vl' (sregs ctx rl)).
+Proof.
+  induction rl; simpl; intros.
+  apply agree_regs_init.
+  inv H. apply agree_regs_init.
+  apply agree_set_reg; auto. 
+Qed.
+
+
+(** ** Executing sequences of moves *)
+
+Lemma tr_moves_init_regs:
+  forall F stk f sp m ctx1 ctx2, context_below ctx1 ctx2 ->
+                                 forall rdsts rsrcs vl pc1 pc2 rs1,
+                                   tr_moves f.(fn_code) pc1 (sregs ctx1 rsrcs) (sregs ctx2 rdsts) pc2 ->
+                                   (forall r, In r rdsts -> Ple r ctx2.(mreg)) ->
+                                   list_forall2 (val_reg_charact F ctx1 rs1) vl rsrcs ->
+                                   exists rs2,
+                                     star step tge (State stk f sp pc1 rs1 m)
+                                          E0 (State stk f sp pc2 rs2 m)
+                                     /\ agree_regs F ctx2 (init_regs vl rdsts) rs2
+                                     /\ forall r, Plt r ctx2.(dreg) -> rs2#r = rs1#r.
+Proof.
+  induction rdsts; simpl; intros.
+  (* rdsts = nil *)
+  inv H0. exists rs1; split. apply star_refl. split. apply agree_regs_init. auto.
+  (* rdsts = a :: rdsts *)
+  inv H2. inv H0. 
+  exists rs1; split. apply star_refl. split. apply agree_regs_init. auto.
+  simpl in H0. inv H0.
+  exploit IHrdsts; eauto. intros [rs2 [A [B C]]].
+  exists (rs2#(sreg ctx2 a) <- (rs2#(sreg ctx1 b1))).
+  split. eapply star_right. eauto. eapply exec_Iop; eauto. traceEq.
+  split. destruct H3 as [[P Q] | [P Q]].
+  subst a1. eapply agree_set_reg_undef; eauto.
+  eapply agree_set_reg; eauto. rewrite C; auto.  apply context_below_lt; auto.
+  intros. rewrite Regmap.gso. auto. apply sym_not_equal. eapply sreg_below_diff; eauto.
+  destruct H2; discriminate.
+Qed.
 
 (** ** Memory invariants *)
 
@@ -89,164 +262,638 @@ Definition loc_private (F: meminj) (m m': mem) (sp: block) (ofs: Z) : Prop :=
 Definition range_private (F: meminj) (m m': mem) (sp: block) (lo hi: Z) : Prop :=
   forall ofs, lo <= ofs < hi -> loc_private F m m' sp ofs.
 
-Inductive match_globalenvs (F: meminj)(bound: block): Prop :=
-  | mk_match_globalenvs
-      (DOMAIN: forall b, Plt b bound -> F b = Some(b, 0))
-      (IMAGE: forall b1 b2 delta, F b1 = Some(b2, delta) -> Plt b2 bound -> b1 = b2)
-      (SYMBOLS: forall id b, Genv.find_symbol SrcGe id = Some b -> Plt b bound)
-      (FUNCTIONS: forall b fd, Genv.find_funct_ptr SrcGe b = Some fd -> Plt b bound)
-      (VARINFOS: forall b gv, Genv.find_var_info SrcGe b = Some gv -> Plt b bound).
+Lemma range_private_invariant:
+  forall F m m' sp lo hi F1 m1 m1',
+    range_private F m m' sp lo hi ->
+    (forall b delta ofs,
+       F1 b = Some(sp, delta) ->
+       Mem.perm m1 b ofs Max Nonempty ->
+       lo <= ofs + delta < hi ->
+       F b = Some(sp, delta) /\ Mem.perm m b ofs Max Nonempty) ->
+    (forall ofs, Mem.perm m' sp ofs Cur Freeable -> Mem.perm m1' sp ofs Cur Freeable) ->
+    range_private F1 m1 m1' sp lo hi.
+Proof.
+  intros; red; intros. exploit H; eauto. intros [A B]. split; auto.
+  intros; red; intros. exploit H0; eauto. omega. intros [P Q]. 
+  eelim B; eauto.
+Qed.
+
+Lemma range_private_perms:
+  forall F m m' sp lo hi,
+    range_private F m m' sp lo hi ->
+    Mem.range_perm m' sp lo hi Cur Freeable.
+Proof.
+  intros; red; intros. eapply H; eauto.
+Qed.
+
+Lemma range_private_alloc_left:
+  forall F m m' sp' base hi sz m1 sp F1,
+    range_private F m m' sp' base hi ->
+    Mem.alloc m 0 sz = (m1, sp) ->
+    F1 sp = Some(sp', base) ->
+    (forall b, b <> sp -> F1 b = F b) ->
+    range_private F1 m1 m' sp' (base + Zmax sz 0) hi.
+Proof.
+  intros; red; intros. 
+  exploit (H ofs). generalize (Zmax2 sz 0). omega. intros [A B].
+  split; auto. intros; red; intros.
+  exploit Mem.perm_alloc_inv; eauto.
+  destruct (eq_block b sp); intros.
+  subst b. rewrite H1 in H4; inv H4. 
+  rewrite Zmax_spec in H3. destruct (zlt 0 sz); omega.
+  rewrite H2 in H4; auto. eelim B; eauto. 
+Qed.
+
+Lemma range_private_free_left:
+  forall F m m' sp base sz hi b m1,
+    range_private F m m' sp (base + Zmax sz 0) hi ->
+    Mem.free m b 0 sz = Some m1 ->
+    F b = Some(sp, base) ->
+    Mem.inject F m m' ->
+    range_private F m1 m' sp base hi.
+Proof.
+  intros; red; intros. 
+  destruct (zlt ofs (base + Zmax sz 0)) as [z|z].
+  red; split. 
+  replace ofs with ((ofs - base) + base) by omega.
+  eapply Mem.perm_inject; eauto.
+  eapply Mem.free_range_perm; eauto.
+  rewrite Zmax_spec in z. destruct (zlt 0 sz); omega. 
+  intros; red; intros. destruct (eq_block b b0).
+  subst b0. rewrite H1 in H4; inv H4.
+  eelim Mem.perm_free_2; eauto. rewrite Zmax_spec in z. destruct (zlt 0 sz); omega.
+  exploit Mem.mi_no_overlap; eauto. 
+  apply Mem.perm_cur_max. apply Mem.perm_implies with Freeable; auto with mem.
+  eapply Mem.free_range_perm. eauto. 
+  instantiate (1 := ofs - base). rewrite Zmax_spec in z. destruct (zlt 0 sz); omega.
+  eapply Mem.perm_free_3; eauto. 
+  intros [A | A]. congruence. omega. 
+
+  exploit (H ofs). omega. intros [A B]. split. auto.
+  intros; red; intros. eelim B; eauto. eapply Mem.perm_free_3; eauto.
+Qed.
+
+Lemma range_private_extcall:
+  forall F F' m1 m2 m1' m2' sp base hi,
+    range_private F m1 m1' sp base hi ->
+    (forall b ofs p,
+       Mem.valid_block m1 b -> Mem.perm m2 b ofs Max p -> Mem.perm m1 b ofs Max p) ->
+    Mem.unchanged_on (loc_out_of_reach F m1) m1' m2' ->
+    Mem.inject F m1 m1' ->
+    inject_incr F F' ->
+    inject_separated F F' m1 m1' ->
+    Mem.valid_block m1' sp ->
+    range_private F' m2 m2' sp base hi.
+Proof.
+  intros until hi; intros RP PERM UNCH INJ INCR SEP VB.
+  red; intros. exploit RP; eauto. intros [A B].
+  split. eapply Mem.perm_unchanged_on; eauto. 
+  intros. red in SEP. destruct (F b) as [[sp1 delta1] |] eqn:?.
+  exploit INCR; eauto. intros EQ; rewrite H0 in EQ; inv EQ. 
+  red; intros; eelim B; eauto. eapply PERM; eauto. 
+  red. destruct (plt b (Mem.nextblock m1)); auto. 
+  exploit Mem.mi_freeblocks; eauto. congruence.
+  exploit SEP; eauto. tauto. 
+Qed.
+
+
+(** ** Relating global environments *)
+
+Inductive match_globalenvs (F: meminj) (bound: block): Prop :=
+| mk_match_globalenvs
+    (DOMAIN: forall b, Plt b bound -> F b = Some(b, 0))
+    (IMAGE: forall b1 b2 delta, F b1 = Some(b2, delta) -> Plt b2 bound -> b1 = b2)
+    (SYMBOLS: forall id b, Genv.find_symbol ge id = Some b -> Plt b bound)
+    (FUNCTIONS: forall b fd, Genv.find_funct_ptr ge b = Some fd -> Plt b bound)
+    (VARINFOS: forall b gv, Genv.find_var_info ge b = Some gv -> Plt b bound).
+
+Lemma find_function_agree:
+  forall ros rs fd F ctx rs' bound,
+    find_function ge ros rs = Some fd ->
+    agree_regs F ctx rs rs' ->
+    match_globalenvs F bound ->
+    exists fd',
+      find_function tge (sros ctx ros) rs' = Some fd' /\ transf_fundef fenv fd = OK fd'.
+Proof.
+  intros. destruct ros as [r | id]; simpl in *.
+  (* register *)
+  assert (rs'#(sreg ctx r) = rs#r).
+  exploit Genv.find_funct_inv; eauto. intros [b EQ].
+  assert (A: val_inject F rs#r rs'#(sreg ctx r)). eapply agree_val_reg; eauto.
+  rewrite EQ in A; inv A.
+  inv H1. rewrite DOMAIN in H5. inv H5. auto.
+  apply FUNCTIONS with fd. 
+  rewrite EQ in H; rewrite Genv.find_funct_find_funct_ptr in H. auto.
+  rewrite H2. eapply functions_translated; eauto.
+  (* symbol *)
+  rewrite symbols_preserved. destruct (Genv.find_symbol ge id); try discriminate.
+  eapply function_ptr_translated; eauto.
+Qed.
+
+(** ** Relating stacks *)
 
 Inductive match_stacks (mu: SM_Injection) (m m': mem):
-             list stackframe -> list stackframe -> block -> Prop :=
-  | match_stacks_nil: forall bound1 bound
-        (MG: match_globalenvs (as_inj mu) bound1)
-        (BELOW: Ple bound1 bound),
-      match_stacks mu m m' nil nil bound
-  | match_stacks_cons: forall res f sp pc rs stk f' sp' rs' stk' bound ctx
-        (MS: match_stacks_inside mu m m' stk stk' f' ctx sp' rs')
-        (FB: tr_funbody fenv f'.(fn_stacksize) ctx f f'.(fn_code))
-        (AG: agree_regs (as_inj mu) ctx rs rs')
-        (SP: (as_inj mu) sp = Some(sp', ctx.(dstk)))
+  list stackframe -> list stackframe -> block -> Prop :=
+| match_stacks_nil: forall bound1 bound
+                           (MG: match_globalenvs (as_inj mu) bound1)
+                           (BELOW: Ple bound1 bound),
+                      match_stacks mu m m' nil nil bound
+| match_stacks_cons: forall res f sp pc rs stk f' sp' rs' stk' bound ctx
+                            (MS: match_stacks_inside mu m m' stk stk' f' ctx sp' rs')
+                            (FB: tr_funbody fenv f'.(fn_stacksize) ctx f f'.(fn_code))
+                            (AG: agree_regs (as_inj mu) ctx rs rs')
+                            (SP: (as_inj mu) sp = Some(sp', ctx.(dstk)))
 (*locBlockSrc mu sp = true*)
 (*locBlockTrg mu sp' = true*)
-        (PRIV: range_private (as_inj mu) m m' sp' (ctx.(dstk) + ctx.(mstk)) f'.(fn_stacksize))
-        (SSZ1: 0 <= f'.(fn_stacksize) < Int.max_unsigned)
-        (SSZ2: forall ofs, Mem.perm m' sp' ofs Max Nonempty -> 0 <= ofs <= f'.(fn_stacksize))
-        (RES: Ple res ctx.(mreg))
-        (BELOW: Plt sp' bound),
-      match_stacks (mu) m m'
-                   (Stackframe res f (Vptr sp Int.zero) pc rs :: stk)
-                   (Stackframe (sreg ctx res) f' (Vptr sp' Int.zero) (spc ctx pc) rs' :: stk')
-                   bound
-  | match_stacks_untailcall: forall stk res f' sp' rpc rs' stk' bound ctx
-        (MS: match_stacks_inside (mu) m m' stk stk' f' ctx sp' rs')
-        (PRIV: range_private (as_inj mu) m m' sp' ctx.(dstk) f'.(fn_stacksize))
-        (SSZ1: 0 <= f'.(fn_stacksize) < Int.max_unsigned)
-        (SSZ2: forall ofs, Mem.perm m' sp' ofs Max Nonempty -> 0 <= ofs <= f'.(fn_stacksize))
-        (RET: ctx.(retinfo) = Some (rpc, res))
+(PRIV: range_private (as_inj mu) m m' sp' (ctx.(dstk) + ctx.(mstk)) f'.(fn_stacksize))
+(SSZ1: 0 <= f'.(fn_stacksize) < Int.max_unsigned)
+(SSZ2: forall ofs, Mem.perm m' sp' ofs Max Nonempty -> 0 <= ofs <= f'.(fn_stacksize))
+(RES: Ple res ctx.(mreg))
+(BELOW: Plt sp' bound),
+                       match_stacks (mu) m m'
+                                    (Stackframe res f (Vptr sp Int.zero) pc rs :: stk)
+                                    (Stackframe (sreg ctx res) f' (Vptr sp' Int.zero) (spc ctx pc) rs' :: stk')
+                                    bound
+| match_stacks_untailcall: forall stk res f' sp' rpc rs' stk' bound ctx
+                                  (MS: match_stacks_inside (mu) m m' stk stk' f' ctx sp' rs')
+                                  (PRIV: range_private (as_inj mu) m m' sp' ctx.(dstk) f'.(fn_stacksize))
+                                  (SSZ1: 0 <= f'.(fn_stacksize) < Int.max_unsigned)
+                                  (SSZ2: forall ofs, Mem.perm m' sp' ofs Max Nonempty -> 0 <= ofs <= f'.(fn_stacksize))
+                                  (RET: ctx.(retinfo) = Some (rpc, res))
 (*locBlockTrg mu sp' = true*)
-        (BELOW: Plt sp' bound),
-      match_stacks (mu) m m'
-                   stk
-                   (Stackframe res f' (Vptr sp' Int.zero) rpc rs' :: stk')
-                   bound
+(BELOW: Plt sp' bound),
+                             match_stacks (mu) m m'
+                                          stk
+                                          (Stackframe res f' (Vptr sp' Int.zero) rpc rs' :: stk')
+                                          bound
 
 with match_stacks_inside (mu: SM_Injection) (m m': mem):
-        list stackframe -> list stackframe -> function -> context -> block -> regset -> Prop :=
-  | match_stacks_inside_base: forall stk stk' f' ctx sp' rs'
-        (MS: match_stacks (mu) m m' stk stk' sp')
+       list stackframe -> list stackframe -> function -> context -> block -> regset -> Prop :=
+     | match_stacks_inside_base: forall stk stk' f' ctx sp' rs'
+                                        (MS: match_stacks (mu) m m' stk stk' sp')
 (*locBlockTrg mu sp' = true*)(*Maybe*)
-        (RET: ctx.(retinfo) = None)
-        (DSTK: ctx.(dstk) = 0),
-      match_stacks_inside (mu) m m' stk stk' f' ctx sp' rs'
-  | match_stacks_inside_inlined: forall res f sp pc rs stk stk' f' ctx sp' rs' ctx'
-        (MS: match_stacks_inside (mu) m m' stk stk' f' ctx' sp' rs')
-        (FB: tr_funbody fenv f'.(fn_stacksize) ctx' f f'.(fn_code))
-        (AG: agree_regs (as_inj mu) ctx' rs rs')
-        (SP: (as_inj mu) sp = Some(sp', ctx'.(dstk)))
+(RET: ctx.(retinfo) = None)
+(DSTK: ctx.(dstk) = 0),
+                                   match_stacks_inside (mu) m m' stk stk' f' ctx sp' rs'
+     | match_stacks_inside_inlined: forall res f sp pc rs stk stk' f' ctx sp' rs' ctx'
+                                           (MS: match_stacks_inside (mu) m m' stk stk' f' ctx' sp' rs')
+                                           (FB: tr_funbody fenv f'.(fn_stacksize) ctx' f f'.(fn_code))
+                                           (AG: agree_regs (as_inj mu) ctx' rs rs')
+                                           (SP: (as_inj mu) sp = Some(sp', ctx'.(dstk)))
 (*locBlockSrc mu sp = true*)
 (*locBlockTrg mu sp' = true*)
-        (PAD: range_private (as_inj mu) m m' sp' (ctx'.(dstk) + ctx'.(mstk)) ctx.(dstk))
-        (RES: Ple res ctx'.(mreg))
-        (RET: ctx.(retinfo) = Some (spc ctx' pc, sreg ctx' res))
-        (BELOW: context_below ctx' ctx)
-        (SBELOW: context_stack_call ctx' ctx),
-      match_stacks_inside (mu) m m' (Stackframe res f (Vptr sp Int.zero) pc rs :: stk)
-                                 stk' f' ctx sp' rs'.
+(PAD: range_private (as_inj mu) m m' sp' (ctx'.(dstk) + ctx'.(mstk)) ctx.(dstk))
+(RES: Ple res ctx'.(mreg))
+(RET: ctx.(retinfo) = Some (spc ctx' pc, sreg ctx' res))
+(BELOW: context_below ctx' ctx)
+(SBELOW: context_stack_call ctx' ctx),
+                                      match_stacks_inside (mu) m m' (Stackframe res f (Vptr sp Int.zero) pc rs :: stk)
+                                                          stk' f' ctx sp' rs'.
+
+(** Properties of match_stacks *)
+
+Section MATCH_STACKS.
+
+
+  Variable F: SM_Injection.
+  Let Finj := as_inj F.
+  Variables m m': mem.
+
+  Lemma match_stacks_globalenvs:
+    forall stk stk' bound,
+      match_stacks F m m' stk stk' bound -> exists b, match_globalenvs Finj b
+                                                      with match_stacks_inside_globalenvs:
+                                                             forall stk stk' f ctx sp rs', 
+                                                               match_stacks_inside F m m' stk stk' f ctx sp rs' -> exists b, match_globalenvs Finj b.
+  Proof.
+    induction 1; eauto.
+    induction 1; eauto.
+  Qed.
+
+  Lemma match_globalenvs_preserves_globals:
+    forall b, match_globalenvs Finj b -> meminj_preserves_globals ge Finj.
+  Proof.
+    intros. inv H. red. split. eauto. split. eauto.
+    intros. symmetry. eapply IMAGE; eauto.
+  Qed. 
+
+  Lemma match_stacks_inside_globals:
+    forall stk stk' f ctx sp rs', 
+      match_stacks_inside F m m' stk stk' f ctx sp rs' -> meminj_preserves_globals ge Finj.
+  Proof.
+    intros. exploit match_stacks_inside_globalenvs; eauto. intros [b A]. 
+    eapply match_globalenvs_preserves_globals; eauto.
+  Qed.
+
+  Lemma match_stacks_bound:
+    forall stk stk' bound bound1,
+      match_stacks F m m' stk stk' bound ->
+      Ple bound bound1 ->
+      match_stacks F m m' stk stk' bound1.
+  Proof.
+    intros. inv H.
+    apply match_stacks_nil with bound0. auto. eapply Ple_trans; eauto. 
+    eapply match_stacks_cons; eauto. eapply Plt_le_trans; eauto. 
+    eapply match_stacks_untailcall; eauto. eapply Plt_le_trans; eauto. 
+  Qed. 
+
+  Variable F1: SM_Injection.
+  Let Finj1 := as_inj F1.
+  Variables m1 m1': mem.
+  Hypothesis INCR: inject_incr Finj Finj1.
+
+  Lemma match_stacks_invariant:
+    forall stk stk' bound, match_stacks F m m' stk stk' bound ->
+                           forall (INJ: forall b1 b2 delta, 
+                                          Finj1 b1 = Some(b2, delta) -> Plt b2 bound -> Finj b1 = Some(b2, delta))
+                                  (PERM1: forall b1 b2 delta ofs,
+                                            Finj1 b1 = Some(b2, delta) -> Plt b2 bound ->
+                                            Mem.perm m1 b1 ofs Max Nonempty -> Mem.perm m b1 ofs Max Nonempty)
+                                  (PERM2: forall b ofs, Plt b bound ->
+                                                        Mem.perm m' b ofs Cur Freeable -> Mem.perm m1' b ofs Cur Freeable)
+                                  (PERM3: forall b ofs k p, Plt b bound ->
+                                                            Mem.perm m1' b ofs k p -> Mem.perm m' b ofs k p),
+                             match_stacks F1 m1 m1' stk stk' bound
+
+                             with match_stacks_inside_invariant:
+                                    forall stk stk' f' ctx sp' rs1, 
+                                      match_stacks_inside F m m' stk stk' f' ctx sp' rs1 ->
+                                      forall rs2
+                                             (RS: forall r, Plt r ctx.(dreg) -> rs2#r = rs1#r)
+                                             (INJ: forall b1 b2 delta, 
+                                                     Finj1 b1 = Some(b2, delta) -> Ple b2 sp' -> Finj b1 = Some(b2, delta))
+                                             (PERM1: forall b1 b2 delta ofs,
+                                                       Finj1 b1 = Some(b2, delta) -> Ple b2 sp' ->
+                                                       Mem.perm m1 b1 ofs Max Nonempty -> Mem.perm m b1 ofs Max Nonempty)
+                                             (PERM2: forall b ofs, Ple b sp' ->
+                                                                   Mem.perm m' b ofs Cur Freeable -> Mem.perm m1' b ofs Cur Freeable)
+                                             (PERM3: forall b ofs k p, Ple b sp' ->
+                                                                       Mem.perm m1' b ofs k p -> Mem.perm m' b ofs k p),
+                                        match_stacks_inside F1 m1 m1' stk stk' f' ctx sp' rs2.
+
+  Proof.
+    induction 1; intros.
+    (* nil *)
+    apply match_stacks_nil with (bound1 := bound1).
+    inv MG. constructor; auto. 
+    intros. apply IMAGE with delta. eapply INJ; eauto. eapply Plt_le_trans; eauto.
+    auto. auto.
+    (* cons *)
+    apply match_stacks_cons with (ctx := ctx); auto.
+    eapply match_stacks_inside_invariant; eauto.
+    intros; eapply INJ; eauto; xomega. 
+    intros; eapply PERM1; eauto; xomega.
+    intros; eapply PERM2; eauto; xomega.
+    intros; eapply PERM3; eauto; xomega.
+    eapply agree_regs_incr; eauto.
+    eapply range_private_invariant; eauto. 
+    (* untailcall *)
+    apply match_stacks_untailcall with (ctx := ctx); auto. 
+    eapply match_stacks_inside_invariant; eauto.
+    intros; eapply INJ; eauto; xomega.
+    intros; eapply PERM1; eauto; xomega.
+    intros; eapply PERM2; eauto; xomega.
+    intros; eapply PERM3; eauto; xomega.
+    eapply range_private_invariant; eauto. 
+
+    induction 1; intros.
+    (* base *)
+    eapply match_stacks_inside_base; eauto.
+    eapply match_stacks_invariant; eauto. 
+    intros; eapply INJ; eauto; xomega.
+    intros; eapply PERM1; eauto; xomega.
+    intros; eapply PERM2; eauto; xomega.
+    intros; eapply PERM3; eauto; xomega.
+    (* inlined *)
+    apply match_stacks_inside_inlined with (ctx' := ctx'); auto. 
+    apply IHmatch_stacks_inside; auto.
+    intros. apply RS. red in BELOW. xomega. 
+    apply agree_regs_incr with Finj; auto. 
+    apply agree_regs_invariant with rs'; auto. 
+    intros. apply RS. red in BELOW. xomega. 
+    eapply range_private_invariant; eauto.
+    intros. split. eapply INJ; eauto. xomega. eapply PERM1; eauto. xomega.
+    intros. eapply PERM2; eauto. xomega.
+  Qed.
+
+  Lemma match_stacks_empty:
+    forall stk stk' bound,
+      match_stacks F m m' stk stk' bound -> stk = nil -> stk' = nil
+      with match_stacks_inside_empty:
+             forall stk stk' f ctx sp rs,
+               match_stacks_inside F m m' stk stk' f ctx sp rs -> stk = nil -> stk' = nil /\ ctx.(retinfo) = None.
+  Proof.
+    induction 1; intros.
+    auto.
+    discriminate.
+    exploit match_stacks_inside_empty; eauto. intros [A B]. congruence.
+    induction 1; intros.
+    split. eapply match_stacks_empty; eauto. auto.
+    discriminate.
+  Qed.
+
+End MATCH_STACKS.
+
+
+
+(** Preservation by assignment to a register *)
+
+Lemma match_stacks_inside_set_reg:
+  forall F m m' stk stk' f' ctx sp' rs' r v, 
+    match_stacks_inside F m m' stk stk' f' ctx sp' rs' ->
+    match_stacks_inside F m m' stk stk' f' ctx sp' (rs'#(sreg ctx r) <- v).
+Proof.
+  intros. eapply match_stacks_inside_invariant; eauto. 
+  intros. apply Regmap.gso. zify. unfold sreg; rewrite shiftpos_eq. xomega.
+Qed.
+
+(** Preservation by a memory store *)
+
+Lemma match_stacks_inside_store:
+  forall F m m' stk stk' f' ctx sp' rs' chunk b ofs v m1 chunk' b' ofs' v' m1', 
+    match_stacks_inside F m m' stk stk' f' ctx sp' rs' ->
+    Mem.store chunk m b ofs v = Some m1 ->
+    Mem.store chunk' m' b' ofs' v' = Some m1' ->
+    match_stacks_inside F m1 m1' stk stk' f' ctx sp' rs'.
+Proof.
+  intros. 
+  eapply match_stacks_inside_invariant; eauto with mem.
+Qed.
+
+(** Preservation by an allocation *)
+
+Lemma match_stacks_inside_alloc_left:
+  forall F m m' stk stk' f' ctx sp' rs',
+    match_stacks_inside F m m' stk stk' f' ctx sp' rs' ->
+    forall sz m1 b F1 delta,
+      Mem.alloc m 0 sz = (m1, b) ->
+      inject_incr (as_inj F) (as_inj F1) ->
+      (as_inj F1) b = Some(sp', delta) ->
+      (forall b1, b1 <> b -> (as_inj F1) b1 = (as_inj F) b1) ->
+      delta >= ctx.(dstk) ->
+      match_stacks_inside F1 m1 m' stk stk' f' ctx sp' rs'.
+Proof.
+  induction 1; intros.
+  (* base *)
+  eapply match_stacks_inside_base; eauto. 
+  eapply match_stacks_invariant; eauto.
+  intros. destruct (eq_block b1 b).
+  subst b1. rewrite H1 in H4; inv H4. eelim Plt_strict; eauto. 
+  rewrite H2 in H4; auto. 
+  intros. exploit Mem.perm_alloc_inv; eauto. destruct (eq_block b1 b); intros; auto.
+  subst b1. rewrite H1 in H4. inv H4. eelim Plt_strict; eauto. 
+  (* inlined *)
+  eapply match_stacks_inside_inlined; eauto. 
+  eapply IHmatch_stacks_inside; eauto. destruct SBELOW. omega. 
+  eapply agree_regs_incr; eauto.
+  eapply range_private_invariant; eauto. 
+  intros. exploit Mem.perm_alloc_inv; eauto. destruct (eq_block b0 b); intros.
+  subst b0. rewrite H2 in H5; inv H5. elimtype False; xomega. 
+  rewrite H3 in H5; auto. 
+Qed.
+
+(** Preservation by freeing *)
+
+Lemma match_stacks_free_left:
+  forall F m m' stk stk' sp b lo hi m1,
+    match_stacks F m m' stk stk' sp ->
+    Mem.free m b lo hi = Some m1 ->
+    match_stacks F m1 m' stk stk' sp.
+Proof.
+  intros. eapply match_stacks_invariant; eauto.
+  intros. eapply Mem.perm_free_3; eauto. 
+Qed.
+
+Lemma match_stacks_free_right:
+  forall F m m' stk stk' sp lo hi m1',
+    match_stacks F m m' stk stk' sp ->
+    Mem.free m' sp lo hi = Some m1' ->
+    match_stacks F m m1' stk stk' sp.
+Proof.
+  intros. eapply match_stacks_invariant; eauto. 
+  intros. eapply Mem.perm_free_1; eauto. 
+  intros. eapply Mem.perm_free_3; eauto.
+Qed.
+
+Lemma min_alignment_sound:
+  forall sz n, (min_alignment sz | n) -> Mem.inj_offset_aligned n sz.
+Proof.
+  intros; red; intros. unfold min_alignment in H. 
+  assert (2 <= sz -> (2 | n)). intros.
+  destruct (zle sz 1). omegaContradiction.
+  destruct (zle sz 2). auto. 
+  destruct (zle sz 4). apply Zdivides_trans with 4; auto. exists 2; auto.
+  apply Zdivides_trans with 8; auto. exists 4; auto.
+  assert (4 <= sz -> (4 | n)). intros.
+  destruct (zle sz 1). omegaContradiction.
+  destruct (zle sz 2). omegaContradiction.
+  destruct (zle sz 4). auto.
+  apply Zdivides_trans with 8; auto. exists 2; auto.
+  assert (8 <= sz -> (8 | n)). intros.
+  destruct (zle sz 1). omegaContradiction.
+  destruct (zle sz 2). omegaContradiction.
+  destruct (zle sz 4). omegaContradiction.
+  auto.
+  destruct chunk; simpl in *; auto.
+  apply Zone_divide.
+  apply Zone_divide.
+  apply H2; omega.
+Qed.
+
+
+(** Preservation by external calls *)
+
+Section EXTCALL.
+
+  Variables F1 F2: SM_Injection.
+  Let Finj1 := as_inj F1.
+  Let Finj2 := as_inj F2.
+  Variables m1 m2 m1' m2': mem.
+  Hypothesis MAXPERM: forall b ofs p, Mem.valid_block m1 b -> Mem.perm m2 b ofs Max p -> Mem.perm m1 b ofs Max p.
+  Hypothesis MAXPERM': forall b ofs p, Mem.valid_block m1' b -> Mem.perm m2' b ofs Max p -> Mem.perm m1' b ofs Max p.
+  Hypothesis UNCHANGED: Mem.unchanged_on (loc_out_of_reach Finj1 m1) m1' m2'.
+  Hypothesis INJ: Mem.inject Finj1 m1 m1'.
+  Hypothesis INCR: inject_incr Finj1 Finj2.
+  Hypothesis SEP: inject_separated Finj1 Finj2 m1 m1'.
+
+  Lemma match_stacks_extcall:
+    forall stk stk' bound, 
+      match_stacks F1 m1 m1' stk stk' bound ->
+      Ple bound (Mem.nextblock m1') ->
+      match_stacks F2 m2 m2' stk stk' bound
+      with match_stacks_inside_extcall:
+             forall stk stk' f' ctx sp' rs',
+               match_stacks_inside F1 m1 m1' stk stk' f' ctx sp' rs' ->
+               Plt sp' (Mem.nextblock m1') ->
+               match_stacks_inside F2 m2 m2' stk stk' f' ctx sp' rs'.
+  Proof.
+    induction 1; intros.
+    apply match_stacks_nil with bound1; auto. 
+    inv MG. constructor; intros; eauto. 
+    destruct (Finj1 b1) as [[b2' delta']|] eqn:?.
+    exploit INCR; eauto. intros EQ; unfold Finj2 in EQ; rewrite H0 in EQ; inv EQ.
+    eapply IMAGE; eauto. 
+    exploit SEP; eauto. intros [A B]. elim B. red. xomega. 
+    eapply match_stacks_cons; eauto. 
+    eapply match_stacks_inside_extcall; eauto. xomega. 
+    eapply agree_regs_incr; eauto. 
+    eapply range_private_extcall; eauto. red; xomega. 
+    intros. apply SSZ2; auto. apply MAXPERM'; auto. red; xomega.
+    eapply match_stacks_untailcall; eauto. 
+    eapply match_stacks_inside_extcall; eauto. xomega. 
+    eapply range_private_extcall; eauto. red; xomega. 
+    intros. apply SSZ2; auto. apply MAXPERM'; auto. red; xomega.
+    induction 1; intros.
+    eapply match_stacks_inside_base; eauto.
+    eapply match_stacks_extcall; eauto. xomega. 
+    eapply match_stacks_inside_inlined; eauto. 
+    eapply agree_regs_incr; eauto. 
+    eapply range_private_extcall; eauto.
+  Qed.
+
+End EXTCALL.
+
+(** Change of context corresponding to an inlined tailcall *)
+
+Lemma align_unchanged:
+  forall n amount, amount > 0 -> (amount | n) -> align n amount = n.
+Proof.
+  intros. destruct H0 as [p EQ]. subst n. unfold align. decEq. 
+  apply Zdiv_unique with (b := amount - 1). omega. omega.
+Qed.
+
+Lemma match_stacks_inside_inlined_tailcall:
+  forall F m m' stk stk' f' ctx sp' rs' ctx' f,
+    match_stacks_inside F m m' stk stk' f' ctx sp' rs' ->
+    context_below ctx ctx' ->
+    context_stack_tailcall ctx f ctx' ->
+    ctx'.(retinfo) = ctx.(retinfo) ->
+    range_private (as_inj F) m m' sp' ctx.(dstk) f'.(fn_stacksize) ->
+    tr_funbody fenv f'.(fn_stacksize) ctx' f f'.(fn_code) ->
+    match_stacks_inside F m m' stk stk' f' ctx' sp' rs'.
+Proof.
+  intros. inv H.
+  (* base *)
+  eapply match_stacks_inside_base; eauto. congruence. 
+  rewrite H1. rewrite DSTK. apply align_unchanged. apply min_alignment_pos. apply Zdivide_0.
+  (* inlined *)
+  assert (dstk ctx <= dstk ctx'). rewrite H1. apply align_le. apply min_alignment_pos.
+  eapply match_stacks_inside_inlined; eauto. 
+  red; intros. destruct (zlt ofs (dstk ctx)). apply PAD; omega. apply H3. inv H4. xomega. 
+  congruence. 
+  unfold context_below in *. xomega.
+  unfold context_stack_call in *. omega. 
+Qed.
+
+(** ** Relating states *)
 
 Inductive match_states:  SM_Injection -> RTL_core -> mem -> RTL_core -> mem -> Prop :=
-  | match_regular_states: forall mu stk f sp pc rs m stk' f' sp' rs' m' ctx
-        (MS: match_stacks_inside mu m m' stk stk' f' ctx sp' rs')
-        (FB: tr_funbody fenv f'.(fn_stacksize) ctx f f'.(fn_code))
-        (AG: agree_regs (as_inj mu) ctx rs rs')
-        (SP: (as_inj mu) sp = Some(sp', ctx.(dstk)))
-        (MINJ: Mem.inject (as_inj mu) m m')
-        (VB: Mem.valid_block m' sp')
-        (PRIV: range_private (as_inj mu) m m' sp' (ctx.(dstk) + ctx.(mstk)) f'.(fn_stacksize))
-        (SSZ1: 0 <= f'.(fn_stacksize) < Int.max_unsigned)
-        (SSZ2: forall ofs, Mem.perm m' sp' ofs Max Nonempty -> 0 <= ofs <= f'.(fn_stacksize)),
-      match_states mu (RTL_State stk f (Vptr sp Int.zero) pc rs) m
-                   (RTL_State stk' f' (Vptr sp' Int.zero) (spc ctx pc) rs') m'
-  | match_call_states: forall (mu: SM_Injection) stk fd args m stk' fd' args' m'
-        (MS: match_stacks mu m m' stk stk' (Mem.nextblock m'))
-        (FD: transf_fundef fenv fd = OK fd')
-        (VINJ: val_list_inject  (as_inj mu) args args')
-        (MINJ: Mem.inject (as_inj mu) m m'),
-      match_states mu (RTL_Callstate stk fd args) m
-                   (RTL_Callstate stk' fd' args') m'
-  | match_call_regular_states: forall (mu: SM_Injection) stk f vargs m stk' f' sp' rs' m' ctx ctx' pc' pc1' rargs
-        (MS: match_stacks_inside mu m m' stk stk' f' ctx sp' rs')
-        (FB: tr_funbody fenv f'.(fn_stacksize) ctx f f'.(fn_code))
-        (BELOW: context_below ctx' ctx)
-        (NOP: f'.(fn_code)!pc' = Some(Inop pc1'))
-        (MOVES: tr_moves f'.(fn_code) pc1' (sregs ctx' rargs) (sregs ctx f.(fn_params)) (spc ctx f.(fn_entrypoint)))
-        (VINJ: list_forall2 (val_reg_charact (as_inj mu) ctx' rs') vargs rargs)
-        (MINJ: Mem.inject (as_inj mu) m m')
-        (VB: Mem.valid_block m' sp')
-        (PRIV: range_private  (as_inj mu) m m' sp' ctx.(dstk) f'.(fn_stacksize))
-        (SSZ1: 0 <= f'.(fn_stacksize) < Int.max_unsigned)
-        (SSZ2: forall ofs, Mem.perm m' sp' ofs Max Nonempty -> 0 <= ofs <= f'.(fn_stacksize)),
-      match_states mu (RTL_Callstate stk (Internal f) vargs) m
-                   (RTL_State stk' f' (Vptr sp' Int.zero) pc' rs') m'
-  | match_return_states: forall (mu: SM_Injection) stk v m stk' v' m'
-        (MS: match_stacks mu m m' stk stk' (Mem.nextblock m'))
-        (VINJ: val_inject (as_inj mu) v v')
-        (MINJ: Mem.inject (as_inj mu) m m'),
-      match_states mu (RTL_Returnstate stk v) m
-                   (RTL_Returnstate stk' v') m'
-  | match_return_regular_states: forall (mu: SM_Injection)stk v m stk' f' sp' rs' m' ctx pc' or rinfo
-        (MS: match_stacks_inside mu m m' stk stk' f' ctx sp' rs')
-        (RET: ctx.(retinfo) = Some rinfo)
-        (AT: f'.(fn_code)!pc' = Some(inline_return ctx or rinfo))
-        (VINJ: match or with None => v = Vundef | Some r => val_inject (as_inj mu) v rs'#(sreg ctx r) end)
-        (MINJ: Mem.inject (as_inj mu) m m')
-        (VB: Mem.valid_block m' sp')
-        (PRIV: range_private (as_inj mu) m m' sp' ctx.(dstk) f'.(fn_stacksize))
-        (SSZ1: 0 <= f'.(fn_stacksize) < Int.max_unsigned)
-        (SSZ2: forall ofs, Mem.perm m' sp' ofs Max Nonempty -> 0 <= ofs <= f'.(fn_stacksize)),
-      match_states mu (RTL_Returnstate stk v) m
-                   (RTL_State stk' f' (Vptr sp' Int.zero) pc' rs') m'.
+| match_regular_states: forall mu stk f sp pc rs m stk' f' sp' rs' m' ctx
+                               (MS: match_stacks_inside mu m m' stk stk' f' ctx sp' rs')
+                               (FB: tr_funbody fenv f'.(fn_stacksize) ctx f f'.(fn_code))
+                               (AG: agree_regs (as_inj mu) ctx rs rs')
+                               (SP: (as_inj mu) sp = Some(sp', ctx.(dstk)))
+                               (MINJ: Mem.inject (as_inj mu) m m')
+                               (VB: Mem.valid_block m' sp')
+                               (PRIV: range_private (as_inj mu) m m' sp' (ctx.(dstk) + ctx.(mstk)) f'.(fn_stacksize))
+                               (SSZ1: 0 <= f'.(fn_stacksize) < Int.max_unsigned)
+                               (SSZ2: forall ofs, Mem.perm m' sp' ofs Max Nonempty -> 0 <= ofs <= f'.(fn_stacksize)),
+                          match_states mu (RTL_State stk f (Vptr sp Int.zero) pc rs) m
+                                       (RTL_State stk' f' (Vptr sp' Int.zero) (spc ctx pc) rs') m'
+| match_call_states: forall (mu: SM_Injection) stk fd args m stk' fd' args' m'
+                            (MS: match_stacks mu m m' stk stk' (Mem.nextblock m'))
+                            (FD: transf_fundef fenv fd = OK fd')
+                            (VINJ: val_list_inject  (as_inj mu) args args')
+                            (MINJ: Mem.inject (as_inj mu) m m'),
+                       match_states mu (RTL_Callstate stk fd args) m
+                                    (RTL_Callstate stk' fd' args') m'
+| match_call_regular_states: forall (mu: SM_Injection) stk f vargs m stk' f' sp' rs' m' ctx ctx' pc' pc1' rargs
+                                    (MS: match_stacks_inside mu m m' stk stk' f' ctx sp' rs')
+                                    (FB: tr_funbody fenv f'.(fn_stacksize) ctx f f'.(fn_code))
+                                    (BELOW: context_below ctx' ctx)
+                                    (NOP: f'.(fn_code)!pc' = Some(Inop pc1'))
+                                    (MOVES: tr_moves f'.(fn_code) pc1' (sregs ctx' rargs) (sregs ctx f.(fn_params)) (spc ctx f.(fn_entrypoint)))
+                                    (VINJ: list_forall2 (val_reg_charact (as_inj mu) ctx' rs') vargs rargs)
+                                    (MINJ: Mem.inject (as_inj mu) m m')
+                                    (VB: Mem.valid_block m' sp')
+                                    (PRIV: range_private  (as_inj mu) m m' sp' ctx.(dstk) f'.(fn_stacksize))
+                                    (SSZ1: 0 <= f'.(fn_stacksize) < Int.max_unsigned)
+                                    (SSZ2: forall ofs, Mem.perm m' sp' ofs Max Nonempty -> 0 <= ofs <= f'.(fn_stacksize)),
+                               match_states mu (RTL_Callstate stk (Internal f) vargs) m
+                                            (RTL_State stk' f' (Vptr sp' Int.zero) pc' rs') m'
+| match_return_states: forall (mu: SM_Injection) stk v m stk' v' m'
+                              (MS: match_stacks mu m m' stk stk' (Mem.nextblock m'))
+                              (VINJ: val_inject (as_inj mu) v v')
+                              (MINJ: Mem.inject (as_inj mu) m m'),
+                         match_states mu (RTL_Returnstate stk v) m
+                                      (RTL_Returnstate stk' v') m'
+| match_return_regular_states: forall (mu: SM_Injection)stk v m stk' f' sp' rs' m' ctx pc' or rinfo
+                                      (MS: match_stacks_inside mu m m' stk stk' f' ctx sp' rs')
+                                      (RET: ctx.(retinfo) = Some rinfo)
+                                      (AT: f'.(fn_code)!pc' = Some(inline_return ctx or rinfo))
+                                      (VINJ: match or with None => v = Vundef | Some r => val_inject (as_inj mu) v rs'#(sreg ctx r) end)
+                                      (MINJ: Mem.inject (as_inj mu) m m')
+                                      (VB: Mem.valid_block m' sp')
+                                      (PRIV: range_private (as_inj mu) m m' sp' ctx.(dstk) f'.(fn_stacksize))
+                                      (SSZ1: 0 <= f'.(fn_stacksize) < Int.max_unsigned)
+                                      (SSZ2: forall ofs, Mem.perm m' sp' ofs Max Nonempty -> 0 <= ofs <= f'.(fn_stacksize)),
+                                 match_states mu (RTL_Returnstate stk v) m
+                                              (RTL_State stk' f' (Vptr sp' Int.zero) pc' rs') m'.
 
-
+Print REACH_closed.
+About REACH.
 Definition MATCH (d:RTL_core) mu c1 m1 c2 m2:Prop :=
   match_states mu c1 m1 c2 m2 /\
   REACH_closed m1 (vis mu) /\
-  meminj_preserves_globals SrcGe (as_inj mu) /\
-  (forall b, isGlobalBlock SrcGe b = true -> frgnBlocksSrc mu b = true) /\
+  meminj_preserves_globals ge (as_inj mu) /\
+  (forall b, isGlobalBlock ge b = true -> frgnBlocksSrc mu b = true) /\
   sm_valid mu m1 m2 /\
   SM_wd mu /\
-  Mem.inject (as_inj mu) m1 m2 (*/\ 
-  globalfunction_ptr_inject (as_inj mu)*) .
+  Mem.inject (as_inj mu) m1 m2.
 
-(** The simulation proof *)
-Theorem transl_program_correct:
-  forall (R: list_norepet (map fst (prog_defs SrcProg)))
-         entrypoints
-         (entry_points_ok : 
-            forall v1 v2 sig,
-              In (v1, v2, sig) entrypoints -> 
-              exists b f1 f2, 
-                v1 = Vptr b Int.zero 
-                /\ v2 = Vptr b Int.zero
-                /\ Genv.find_funct_ptr SrcGe b = Some f1
-                /\ Genv.find_funct_ptr TrgGe b = Some f2)
-         (init_mem: exists m0, Genv.init_mem SrcProg = Some m0),
-    SM_simulation.SM_simulation_inject rtl_eff_sem
-                                       rtl_eff_sem SrcGe TrgGe entrypoints.
-
-  intros.
-  (*eapply sepcomp.effect_simulations_lemmas.inj_simulation_star_wf.*)
-  Definition RTL_measure (S: RTL_core) : nat :=
+(** ** Forward simulation *)
+Definition RTL_measure (S: RTL_core) : nat :=
   match S with
   | RTL_State _ _ _ _ _ => 1%nat
   | RTL_Callstate _ _ _ => 0%nat
   | RTL_Returnstate _ _ => 0%nat
   end.
+
+
+Lemma tr_funbody_inv:
+  forall sz cts f c pc i,
+    tr_funbody fenv sz cts f c -> f.(fn_code)!pc = Some i -> tr_instr fenv sz cts pc i c.
+Proof.
+  intros. inv H. eauto. 
+Qed.
+
+(** MISSING THEOREM step_simulation *)
+
+
+Definition entry_points_ok entrypoints:= forall (v1 v2 : val) (sig : signature),
+                                             In (v1, v2, sig) entrypoints -> 
+                                             exists b f1 f2, 
+                                               v1 = Vptr b Int.zero 
+                                               /\ v2 = Vptr b Int.zero
+                                               /\ Genv.find_funct_ptr ge b = Some f1
+                                               /\ Genv.find_funct_ptr tge b = Some f2.
+
+(** ** Behold the theorem *)
+Theorem transl_program_correct:
+  forall (R: list_norepet (map fst (prog_defs SrcProg)))
+         (entrypoints : list (val * val * signature))
+         (entry_ok : entry_points_ok entrypoints)
+         (init_mem: exists m0, Genv.init_mem SrcProg = Some m0),
+    SM_simulation.SM_simulation_inject rtl_eff_sem
+                                       rtl_eff_sem ge tge entrypoints.
+
+
+  intros.
+  (*eapply sepcomp.effect_simulations_lemmas.inj_simulation_star_wf.*)
   eapply sepcomp.effect_simulations_lemmas.inj_simulation_star with (match_states:= MATCH)(measure:= RTL_measure).
 
   Lemma environment_equality: (exists m0:mem, Genv.init_mem SrcProg = Some m0) -> 
-                                     genvs_domain_eq SrcGe TrgGe.
+                                     genvs_domain_eq ge tge.
     descend;
     destruct H0 as [b0]; exists b0;
     rewriter_back;
@@ -268,16 +915,6 @@ Theorem transl_program_correct:
   Hint Resolve MATCH_RC: trans_correct.
   eauto with trans_correct.
 
-  (*Lemma restrict_preserves_globalfun_ptr: forall j X
-  (PG : globalfunction_ptr_inject j)
-  (Glob : forall b, isGlobalBlock SrcGe b = true -> X b = true),
-globalfunction_ptr_inject (restrict j X).
-Proof. intros.
-  red; intros. 
-  destruct (PG _ _ H). split; trivial.
-  apply restrictI_Some; try eassumption.
-  apply (Glob _ H1).
-Qed.*)
 
 Lemma MATCH_restrict: forall (d : RTL_core) (mu : SM_Injection) (c1 : RTL_core) 
                                  (m1 : mem) (c2 : RTL_core) (m2 : mem) (X : block -> bool) (MC: MATCH d mu c1 m1 c2 m2)(HX: forall b : block, vis mu b = true -> X b = true)(RC0:REACH_closed m1 X), MATCH d (restrict_sm mu X) c1 m1 c2 m2.
@@ -294,8 +931,9 @@ Lemma match_states_restrict: forall mu m1 m2 c1 c2 X
       (RC: REACH_closed m1 X)
       (MCS: match_states mu c1 m1 c2 m2 ),
       match_states (restrict_sm mu X) c1 m1 c2 m2.
-admit.
+  admit.
 Qed.
+
 apply match_states_restrict; intuition.
 
 split. unfold vis.
@@ -334,12 +972,12 @@ eauto with trans_correct.
 Lemma MATCH_PG:  forall (d : RTL_core) (mu : SM_Injection) (c1 : RTL_core) 
                                            (m1 : mem) (c2 : RTL_core) (m2 : mem)(
                                       MC: MATCH d mu c1 m1 c2 m2),
-                                      meminj_preserves_globals SrcGe (extern_of mu) /\
+                                      meminj_preserves_globals ge (extern_of mu) /\
                                       (forall b : block,
-                                         isGlobalBlock SrcGe b = true -> frgnBlocksSrc mu b = true).
+                                         isGlobalBlock ge b = true -> frgnBlocksSrc mu b = true).
 Proof.
   intros.
-  assert (GF: forall b, isGlobalBlock SrcGe b = true -> frgnBlocksSrc mu b = true).
+  assert (GF: forall b, isGlobalBlock ge b = true -> frgnBlocksSrc mu b = true).
     apply MC.
   split; trivial.
   rewrite <- match_genv_meminj_preserves_extern_iff_all; trivial.
@@ -349,40 +987,34 @@ Hint Resolve MATCH_PG: trans_correct.
 eauto with trans_correct.
 
 Lemma MATCH_initial_core: forall (v1 v2 : val) (sig : signature) entrypoints
-  (entry_points_ok : forall (v1 v2 : val) (sig : signature),
-                    In (v1, v2, sig) entrypoints ->
-                    exists (b : block) (f1 f2 : fundef),
-                      v1 = Vptr b Int.zero /\
-                      v2 = Vptr b Int.zero /\
-                      Genv.find_funct_ptr SrcGe b = Some f1 /\
-                      Genv.find_funct_ptr TrgGe b = Some f2)
+  (entry_ok : entry_points_ok entrypoints)
    (EP: In (v1, v2, sig) entrypoints)
    (vals1 : list val) (c1 : RTL_core) (m1 : mem) 
      (j : meminj) (vals2 : list val) (m2 : mem) (DomS DomT : block -> bool)
-   (SM_Ini:initial_core rtl_eff_sem SrcGe v1 vals1 = Some c1)
+   (SM_Ini:initial_core rtl_eff_sem ge v1 vals1 = Some c1)
    (Inj: Mem.inject j m1 m2)
    (VInj: Forall2 (val_inject j) vals1 vals2)
-   (PG: meminj_preserves_globals SrcGe j)
+   (PG: meminj_preserves_globals ge j)
    (J: forall (b1 b2 : block) (d : Z),
     j b1 = Some (b2, d) -> DomS b1 = true /\ DomT b2 = true)
    (RCH: forall b : block,
-    REACH m2 (fun b' : block => isGlobalBlock TrgGe b' || getBlocks vals2 b')
+    REACH m2 (fun b' : block => isGlobalBlock tge b' || getBlocks vals2 b')
       b = true -> DomT b = true)
    (HDomS: (forall b : block, DomS b = true -> Mem.valid_block m1 b))
    (HDomT: (forall b : block, DomT b = true -> Mem.valid_block m2 b)),
    exists c2 : RTL_core,
-     initial_core rtl_eff_sem TrgGe v2 vals2 = Some c2 /\
+     initial_core rtl_eff_sem tge v2 vals2 = Some c2 /\
      MATCH c1
        (initial_SM DomS DomT DomS DomT j) (*
           (REACH m1
-             (fun b : block => isGlobalBlock SrcGe b || getBlocks vals1 b))
+             (fun b : block => isGlobalBlock ge b || getBlocks vals1 b))
           (REACH m2
-             (fun b : block => isGlobalBlock TrgGe b || getBlocks vals2 b)) j)*)
+             (fun b : block => isGlobalBlock tge b || getBlocks vals2 b)) j)*)
        c1 m1 c2 m2.
  Proof.
   intros.
   inversion SM_Ini.
-  unfold  RTL_initial_core in H0. unfold SrcGe in *. unfold TrgGe in *.
+  unfold  RTL_initial_core in H0. unfold ge in *. unfold tge in *.
   destruct v1; inv H0.
   remember (Int.eq_dec i Int.zero) as z; destruct z; inv H1. clear Heqz.
   remember (Genv.find_funct_ptr (Genv.globalenv SrcProg) b) as zz; destruct zz; inv H0. 
@@ -391,16 +1023,15 @@ Lemma MATCH_initial_core: forall (v1 v2 : val) (sig : signature) entrypoints
   exists (RTL_Callstate nil tf vals2).
   split. 
   simpl. 
-  destruct (entry_points_ok _ _ _ EP) as [b0 [f1 [f2 [A [B [C D]]]]]].
-  subst. inv A. rewrite C in Heqzz. inv Heqzz. 
-  unfold SrcGe, TrgGe in *.
+  destruct (entry_ok _ _ _ EP) as [b0 [f1 [f2 [A [B [C D]]]]]].
+  subst. inv A.
+  unfold ge, tge in *. rewrite C in Heqzz. inv Heqzz. 
   rewrite D in FIND. inv FIND.
   unfold RTL_initial_core. 
   case_eq (Int.eq_dec Int.zero Int.zero). intros ? e.
   solve[rewrite D; auto].
   intros CONTRA.
   solve[elimtype False; auto].
-  (*destruct InitMem as [m0 [INIT_MEM [A B]]].*)
   admit.
 Qed.
 Hint Resolve MATCH_initial_core: trans_correct.
@@ -534,8 +1165,8 @@ assert (PHnu': meminj_preserves_globals (Genv.globalenv SrcProg) (as_inj nu')).
       apply joinI; left. apply INC.
       rewrite replace_locals_extern.
       apply foreign_in_extern.
-     assert (GG: isGlobalBlock SrcGe b = true).
-          unfold isGlobalBlock, SrcGe. apply genv2blocksBool_char1 in H.
+     assert (GG: isGlobalBlock ge b = true).
+          unfold isGlobalBlock, ge. apply genv2blocksBool_char1 in H.
           rewrite H. trivial.
       Check frgnSrc.
       destruct (frgnSrc _ WDmu _ (GF _ GG)) as [bb2 [dd [FF FT2]]].
@@ -544,8 +1175,8 @@ assert (PHnu': meminj_preserves_globals (Genv.globalenv SrcProg) (as_inj nu')).
     split; intros. specialize (PGb _ H).
       apply joinI; left. apply INC.
       rewrite replace_locals_extern. 
-      assert (GG: isGlobalBlock SrcGe b = true). (*4 goals*)
-          unfold isGlobalBlock, SrcGe. apply genv2blocksBool_char2 in H.
+      assert (GG: isGlobalBlock ge b = true). (*4 goals*)
+          unfold isGlobalBlock, ge. apply genv2blocksBool_char2 in H.
           rewrite H. intuition. (*3 goals*)
       destruct (frgnSrc _ WDmu _ (GF _ GG)) as [bb2 [dd [FF FT2]]].
       rewrite (foreign_in_all _ _ _ _ FF) in PGb. inv PGb.
@@ -676,81 +1307,8 @@ split.
   unfold vis in *.
   rewrite replace_externs_frgnBlocksSrc, replace_externs_locBlocksSrc in *.
   econstructor; try eassumption.
-
-(*
-Lemma structured_match_callstack_incr_bound:
-  forall f m tm cs bound tbound bound' tbound',
-  match_stacks f m tm cs bound (*tbound*) ->
-  Ple bound bound' -> Ple tbound tbound' ->
-  match_stacks f m tm cs bound' tbound'.
-Proof.
-  intros. inv H.
-  econstructor; eauto. xomega. xomega. 
-  constructor; auto. xomega. xomega.
-
-
-
-    eapply structured_match_callstack_incr_bound.
-Lemma structured_match_callstack_ext: forall mu m1 m2 cs bound 
-  tbound
-  (MCS : match_stacks mu m1 m2 cs bound tbound)
-  m1' (FwdSrc : mem_forward m1 m1')
-  nu vals1 vals2
-  (Hnu: nu = replace_locals mu
-                      (fun b0 : Values.block =>
-                       locBlocksSrc mu b0 &&
-                       REACH m1 (exportedSrc mu vals1) b0)
-                      (fun b0 : Values.block =>
-                       locBlocksTgt mu b0 &&
-                       REACH m2 (exportedTgt mu vals2) b0))
-  (SMvalMu : sm_valid mu m1 m2)
-  (PG : meminj_preserves_globals (Genv.globalenv SrcProg) (as_inj mu))
-  nu' (INC : extern_incr nu nu')
-  (SEP : sm_inject_separated nu nu' m1 m2)
-  (UNMAPPED : Mem.unchanged_on
-                (fun (b : Values.block) (_ : Z) =>
-                 locBlocksSrc nu b = true /\ pubBlocksSrc nu b = false) m1
-                m1')
-   m2' (FwdTgt : mem_forward m2 m2') (OUTOFREACH : Mem.unchanged_on (local_out_of_reach nu m1) m2 m2')
-  ret1 ret2 (WDnu' : SM_wd nu') (WDmu : SM_wd mu) (WDnu : SM_wd nu)
-  (BND: Ple bound (Mem.nextblock m1))
-  (TBND:Ple tbound (Mem.nextblock m2)),
-match_stacks
-  (replace_externs nu'
-        (fun b : Values.block =>
-         DomSrc nu' b &&
-         (negb (locBlocksSrc nu' b) && REACH m1' (exportedSrc nu' (ret1 :: nil)) b))
-        (fun b : Values.block =>
-         DomTgt nu' b &&
-         (negb (locBlocksTgt nu' b) && REACH m2' (exportedTgt nu' (ret2 :: nil)) b)))
-   m1' m2' cs bound tbound.
-Proof.
-
-
-
-      eapply structured_match_callstack_ext with
-       (mu:=mu)(nu':=nu'); try reflexivity; try eassumption.
-       eapply eff_after_check1 with (mu:=mu); try eassumption; try reflexivity.
-         eapply forall_vals_inject_restrictD; eassumption.
-       apply (forward_nextblock _ _ FwdSrc).
-       apply (forward_nextblock _ _ FwdTgt).*)
-admit.
-
-    rewrite replace_externs_as_inj. assumption.
-    (*Check restrict_val_inject.
-    eapply restrict_val_inject; try eassumption.
-    Print restrict_val_inject.
-      (*eapply restrict_val_inject; try eassumption.*)
-    intros.
-        destruct (getBlocks_inject (as_inj nu') (ret1::nil) (ret2::nil))
-           with (b:=b) as [bb [dd [JJ' GBbb]]]; try eassumption.
-          constructor. assumption. constructor.
-         unfold vis. rewrite replace_externs_frgnBlocksSrc, replace_externs_locBlocksSrc.
-        remember (locBlocksSrc nu' b) as d.
-        destruct d; simpl; trivial. apply andb_true_iff.
-        split. eapply as_inj_DomRng; eassumption.
-        apply REACH_nil. unfold exportedSrc.
-           rewrite H. trivial.*)
+  admit.
+  rewrite replace_externs_as_inj. assumption.
 admit.
 unfold vis.
 rewrite replace_externs_locBlocksSrc, replace_externs_frgnBlocksSrc,
@@ -763,580 +1321,714 @@ Qed.
 Hint Resolve Match_AfterExternal: trans_correct.
 eauto with trans_correct.
 
-Focus 1.
+clear entry_ok.
+clear init_mem.
 
 
-intros.
-simpl in *.
-destruct H0.
-Print match_states.
+Ltac extend_smart:=  let x := fresh "x" in extensionality x.
+  Ltac rewrite_freshloc := match goal with
+                             | H: (Mem.storev _ _ _ _ = Some _) |- _ => rewrite (storev_freshloc _ _ _ _ _ H)
+                             | H: (Mem.free _ _ _ _ = Some _) |- _ => apply freshloc_free in H; rewrite H
+                             | _ => try rewrite freshloc_irrefl
+                           end.
+  Ltac loc_alloc_solve := apply sm_locally_allocatedChar; repeat split; try extend_smart;
+                          try rewrite_freshloc; intuition.
+Print sm_locally_allocated.
 
-inv H.
-inv H0.
+  Lemma step_simulation_noeffect: forall (st1 : RTL_core) (m1 : mem) (st1' : RTL_core) (m1' : mem)
+                                         (CS: corestep rtl_eff_sem ge st1 m1 st1' m1')
+                                         (st2 : RTL_core) (mu : SM_Injection) (m2 : mem)
+                                         (MC:MATCH st1 mu st1 m1 st2 m2),
+                                  exists (st2' : RTL_core) (m2' : mem),
+                                    (corestep_plus rtl_eff_sem tge st2 m2 st2' m2' \/
+                                     (RTL_measure st1' < RTL_measure st1)%nat /\
+                                     corestep_star rtl_eff_sem tge st2 m2 st2' m2') /\
+                                    exists (mu' : SM_Injection),
+                                      intern_incr mu mu' /\
+                                      sm_inject_separated mu mu' m1 m2 /\
+                                      sm_locally_allocated mu mu' m1 m2 m1' m2' /\
+                                      MATCH st1' mu' st1' m1' st2' m2'.
+    
+    intros.
+    simpl in *.
+    destruct MC as [MS H].
+    
+    inv CS;
+      inv MS.
+    (* Inop *)
+    exploit tr_funbody_inv; eauto. intros TR; inv TR.
+    eexists. eexists. 
 
-eexists. 
-eexists. exists mu.
-intuition.
-apply intern_incr_refl.
-apply sm_inject_separated_same_sminj.
-apply sm_locally_allocatedChar.
-repeat split; extensionality b;
-rewrite freshloc_irrefl;
-intuition.
-(*unfold MATCH.
-intuition.
-eapply match_regular_states; first [eassumption| split; eassumption].
-(*unfold RTL_measure; simpl.*)*)
-Focus 2.
-left.
-eapply rtl_corestep_exec_Inop in H2.
-
-unfold corestep_plus, corestepN. simpl.
-exists O. eexists. eexists.
-simpl.
-split.
-eapply H2.
-Print RTL_corestep.
-eapply H9.
-
-Lemma RTL_corestep_plus_one: forall (ge : genv) (c c' : RTL_core) (m m' : mem),
-    RTL_corestep ge c m c' m' -> corestep_plus RTL_core_sem ge c m c' m'.
-Admitted.
-apply RTL_corestep_plus_one. eapply H9.
-
-
-RTL_corestep
-     : genv -> RTL_core -> mem -> RTL_core -> mem -> Prop.
-
-eassumption.
-
-
-Print RTL_State.
-Focus 1.
-
-assert (spc ctx pc = (spc ctx pc')).
-unfold spc. unfold shiftpos.
-Print Pos.pred.
-
-f_equal.
-Locate "+".
-Print Pos.add.
-
-Print State.
-
-(* apply match_regular_states. *)
-Print match_states.
-
-Print spc.
-Check ctx.
-
-
-destruct H.
- 
-(* match_regular_states *)
-eapply match_regular_states.
-(*match_call_states*)
-
-(* match_call_regular_states *)
-
-(* match_return_states *)
-
-(* match_return_regular_states *)
-unfold match_states.
-eapply exec_Inop in H.
- inv H.
-simpl in *.
-Print RTL_corestep.
-induction H; simpl in *.
-Focus 1.
-intuition.
-
-
-
-
-
-
-
-split; intuition.
-destruct sp0. 
-eapply match_regular_states; eauto.
-
-econstructor.
-
-
-
-Ltac openHyp:= match goal with
-                     | [H: and _ _ |- _] => destruct H
-                     | [H: exists _, _ |- _] => destruct H
-                 end.
-
-(*Lemma MS_step_case_SkipSeq: forall 
-(MCS : structured_match_callstack mu m tm
-               (Frame cenv tfn e lenv te sp lo hi :: cs)
-               (Mem.nextblock m)
-               (Mem.nextblock tm))
-(MK : match_cont (Csharpminor.Kseq s k) tk cenv xenv cs),
-exists st2' : CMin_core, 
-  exists m2' mu',
-   corestep_plus CMin_core_sem tge
-     (CMin_State tfn Sskip tk (Vptr sp Int.zero) te) tm st2' m2' 
-  /\ intern_incr mu mu' /\
-  sm_inject_separated mu mu' m tm /\
-  sm_locally_allocated mu mu' m tm m m2' /\
-  Match_cores (CSharpMin_State f s k e lenv) mu'
-    (CSharpMin_State f s k e lenv) m st2' m2' /\
-  SM_wd mu' /\ sm_valid mu' m m2'.*)
-
-Admitted.
-
-
-Lemma corestep_plus_star: 
-   forall (st1 : RTL_core) (m1 : mem) (st1' : RTL_core) (m1' : mem)
-   (CS: corestep rtl_eff_sem SrcGe st1 m1 st1' m1')
-   (st2 : RTL_core) (mu : SM_Injection) (m2 : mem)
-   (MC: MATCH st1 mu st1 m1 st2 m2),
-   exists (st2' : RTL_core) (m2' : mem) (mu' : SM_Injection),
-     intern_incr mu mu' /\
-     sm_inject_separated mu mu' m1 m2 /\
-     sm_locally_allocated mu mu' m1 m2 m1' m2' /\
-     MATCH st1' mu' st1' m1' st2' m2' /\
-     (*SM_wd mu' /\
-     sm_valid mu' m1' m2' /\*)
-     (corestep_plus rtl_eff_sem TrgGe st2 m2 st2' m2' \/
-      (RTL_measure st1' < RTL_measure st1)%nat /\
-      corestep_star rtl_eff_sem TrgGe st2 m2 st2' m2').
-intros.
-inv CS.
-
-(*Skip *)
-      destruct MC as [SMC PRE].
-      Check match_states.
-      inv SMC; simpl in *.
-      Check match_cont.
-  dependent induction MK.
-
-  eexists. eexists. exists mu. 
-  split.
-    apply corestep_plus_one. 
-        econstructor. 
-  simpl. (* exists (CSharpMin_State f s k e le).
-     left. *) intuition. 
+    split.
+    left.
+    eapply corestep_plus_one.
+    eapply rtl_corestep_exec_Inop. eassumption.
+    exists mu.
+    intuition.
     apply intern_incr_refl.
     apply sm_inject_separated_same_sminj.
-    apply sm_locally_allocatedChar.
-      repeat split; extensionality b; 
-      try rewrite freshloc_irrefl; intuition.
-    split; intuition.
-    eapply SMC_states; eauto. 
+    loc_alloc_solve.
+    unfold MATCH.
+    intuition.
+    eapply match_regular_states; first [eassumption| split; eassumption].
 
-  eexists. eexists. exists mu. 
-  split.
-    apply corestep_plus_one. 
-        econstructor. 
-   simpl. (*exists (CSharpMin_State f (Csharpminor.Sseq s1 s2) k e le).
-      left.  *) intuition. 
+
+    (* Iop *)
+    Focus 1.
+    exploit tr_funbody_inv; eauto. intros TR; inv TR.
+    repeat open_Hyp.
+    exploit eval_operation_inject. 
+
+    eapply match_stacks_inside_globals; eauto.
+    exact SP.
+    instantiate (2 := rs##args). instantiate (1 := rs'##(sregs ctx args)). eapply agree_val_regs; eauto.
+    eexact MINJ. eauto.
+    fold (sop ctx op). intros [v' [A B]].
+    eexists. eexists.
+    split; simpl.
+    left. 
+    eapply corestep_plus_one. 
+
+    eapply rtl_corestep_exec_Iop. eassumption.
+    erewrite eval_operation_preserved; eauto.
+    exact symbols_preserved. 
+    econstructor; eauto. 
+    intuition.
     apply intern_incr_refl.
     apply sm_inject_separated_same_sminj.
-    apply sm_locally_allocatedChar.
-      repeat split; extensionality b; 
-      try rewrite freshloc_irrefl; intuition.
-    split; intuition.
-    eapply SMC_state_seq; eauto.
-
-  exploit IHMK; eauto. clear IHMK. 
-  intros [T2 [m2 [nu [A C]]]].
-  exists T2. exists m2. exists nu. 
-  split.
-     eapply corestep_star_plus_trans.
-        apply corestep_star_one. 
-        constructor.
-        simpl. apply A. 
-  apply C.
+    loc_alloc_solve.
+    unfold MATCH.
+    intuition.
+    eapply match_regular_states; eauto.
 
 
+    apply match_stacks_inside_set_reg; auto.
+    apply agree_set_reg; auto. 
 
 
-
-
-      
-      (*monadInv TR.*)
-      destruct (MS_step_case_SkipSeq _ _ _ _ _ _ _ _ _ _ _ _ _ _ _ _ _ _ 
-        PRE TRF MCS MK) as [c2' [m2' [mu' [cstepPlus MS]]]].
-      exists c2'. exists m2'. exists mu'. 
+    (* Iload *)
+    exploit tr_funbody_inv; eauto. intros TR; inv TR.
+    exploit eval_addressing_inject. 
+    eapply match_stacks_inside_globals; eauto.
+    eexact SP.
+    instantiate (2 := rs##args). instantiate (1 := rs'##(sregs ctx args)). eapply agree_val_regs; eauto.
+    eauto.
+    fold (saddr ctx addr). intros [a' [P Q]].
+    exploit Mem.loadv_inject; eauto. intros [v' [U V]].
+    assert (eval_addressing tge (Vptr sp' Int.zero) (saddr ctx addr) rs' ## (sregs ctx args) = Some a').
+    rewrite <- P. apply eval_addressing_preserved. exact symbols_preserved.
+    eexists. eexists.
+    split; simpl. left.
+    eapply corestep_plus_one. 
+    eapply rtl_corestep_exec_Iload; try eassumption.
+    exists mu.
+    intuition.
+    apply intern_incr_refl.
+    apply sm_inject_separated_same_sminj.
+    loc_alloc_solve.
+    unfold MATCH;
       intuition.
-destruct MC as []
-unfold corestep in *.
-unfold core_data in *.
-Check exploit.
-exploit Match_corestep; eauto.
-    intros [? [? [? [? [? [? [? [? [? ?]]]]]]]]].
-    exists x, x0, x1.
-    split; auto.
-
-inv MC; 
-repeat openHyp.
-inv H.
- intros.
-    exploit Match_corestep; eauto.
-    intros [? [? [? [? [? [? [? [? [? ?]]]]]]]]].
-    exists x, x0, x1.
-    split; auto.
-
-eapply corestep_plus_star; auto.
-intros.
-inv MC.
-inv H; simpl in *.
-
-SearchAbout intern_incr.
-
-
-unfold   well_founded.
-Print Acc.
-
-
-
-
-
-
-
-
-
-
-
-
-
-
-
-
-
-
-
-
-
-
-
-
-
-
-
-
-
-
-
-
-
-
-Lemma inject_val_inject_halted: forall (cd : RTL_core) (mu : SM_Injection) (c1 : RTL_core) 
-                                       (m1 : mem) (c2 : RTL_core) (m2 : mem) (v1 : val) (MC: MATCH cd mu c1 m1 c2 m2) (Hl: halted rtl_eff_sem c1 = Some v1 ),
-                                  exists v2 : val,
-                                    Mem.inject (as_inj mu) m1 m2 /\
-                                    val_inject (restrict (as_inj mu) (vis mu)) v1 v2 /\
-                                    halted rtl_eff_sem c2 = Some v2.
-Proof.
-intros. 
-eexists.
-unfold MATCH in MC.
-destruct MC as [? MC].
-inv H. simpl in *. inv Hl.  
-destruct 
-split; [|split].
-unfold Mem.inject.
-eapply MC.
-
-{ intros. destruct H as [MC [RC [PG [GF [VAL [WD INJ]]]]]]. 
-    eapply MATCH_safely_halted in MC; eauto.
-    destruct MC as [v2 [A B]].
-    exists v2. intuition. }
-
-
-unfold MATCH in MC.  
-
-
-
-
-
-
-
-
-
-
-
-
-
-
-(*Old proof*)
-  inversion Ini.
-  unfold RTL_initial_core in H0. unfold ge in *. unfold TrgGe in *.
-  destruct v1; inv H0.
-  remember (Int.eq_dec i Int.zero) as z; destruct z; inv H1. clear Heqz.
-  remember (Genv.find_funct_ptr (Genv.globalenv SrcProg) b) as zz; destruct zz; inv H0. 
-    apply eq_sym in Heqzz.
-
-  (*exploit function_ptr_translated; eauto.*)
-  destruct (entry_points_ok _ _ _ EP) as [b0 [f1 [f2 [A [B [C D]]]]]].
-  eexists (RTL_Callstate nil _ vals2).
-  split.
-    subst. inv A. unfold SrcGe in C. rewrite C in Heqzz. inv Heqzz.
-    unfold rtl_eff_sem (*, RTL_coop_sem*). simpl.
-    case_eq (Int.eq_dec Int.zero Int.zero). intros ? e.
-    solve[rewrite D; auto].
-    intros CONTRA.
-    solve[elimtype False; auto].
-(*  assert (exists targs tres, type_of_fundef f = Tfunction targs tres).
-         destruct f; simpl. eexists; eexists. reflexivity.
-         eexists; eexists. reflexivity.
-  destruct H as [targs [tres Tfun]].*)
-  destruct (core_initial_wd SrcGe TrgGe _ _ _ _ _ _ _  Inj
-     VInj J RCH PG GDE HDomS HDomT _ (eq_refl _))
-    as [AA [BB [CC [DD [EE [FF GG]]]]]].
-  split.
-  simpl in Ini.
-  (* There is a better way to do this *)
-  destruct Int.eq_dec in Ini; [destruct Genv.find_funct_ptr in Ini| ]; [ |discriminate | discriminate].
-  inversion Ini.
-    eapply match_call_states; try eassumption.
-    eapply match_stacks_nil.
-    unfold match_globalenvs.
-      constructor.
-      rewrite initial_SM_as_inj.
-        unfold vis, initial_SM; simpl.
-        apply forall_inject_val_list_inject.
-        eapply restrict_forall_vals_inject; try eassumption.
-          intros. apply REACH_nil. rewrite H; intuition.
-    rewrite initial_SM_as_inj.
-      unfold vis, initial_SM; simpl.
-      eapply inject_restrict; eassumption.
-  intuition.
-    rewrite match_genv_meminj_preserves_extern_iff_all.
-      assumption.
-      apply BB.
-      apply EE.
-    (*as in selectionprffEFF*)
-    rewrite initial_SM_as_inj.
-      red; intros. specialize (Genv.find_funct_ptr_not_fresh prog). intros.
-         destruct InitMem as [m0 [INIT_MEM [? ?]]].
-         specialize (H0 _ _ _ INIT_MEM H). 
-         destruct (valid_init_is_global _ R _ INIT_MEM _ H0) as [id Hid]. 
-           destruct PG as [PGa [PGb PGc]]. split. eapply PGa; eassumption.
-         unfold isGlobalBlock. 
-          apply orb_true_iff. left. apply genv2blocksBool_char1.
-            simpl. exists id; eassumption.
-    rewrite initial_SM_as_inj; assumption.
-Qed.
-
-
-
-
-apply MATCH_REACH_REACH.
-
-apply inject_val_inject_halted.
-
-
-
-Record map_wf (m: mapping) : Prop :=
-  mk_map_wf {
-      map_wf_inj:
-        (forall id1 id2 r,
-           m.(map_vars)!id1 = Some r -> m.(map_vars)!id2 = Some r -> id1 = id2);
-      map_wf_disj:
-        (forall id r,
-           m.(map_vars)!id = Some r -> In r m.(map_letvars) -> False)
-    }.
-
-Inductive match_states (j:meminj): CMinSel_core -> mem -> RTL_core -> mem -> Prop :=
-| match_state:
-    forall f s k sp e m tm cs tf ns rs map ncont nexits ngoto nret rret sp'
-           (MWF: map_wf map)
-           (TS: tr_stmt tf.(fn_code) map s ns ncont nexits ngoto nret rret)
-           (TF: tr_fun tf map f ngoto nret rret)
-           (TK: tr_cont j tf.(fn_code) map k ncont nexits ngoto nret rret cs)
-           (ME: match_env j map e nil rs)
-        (*(MEXT: Mem.extends m tm)*)
-        (MINJ: Mem.inject j m tm)
-                 (*NEW:*) (SP: sp_preserved j sp sp'),
-      match_states j (CMinSel_State f s k sp e) m
-                   (RTL_State cs tf sp' ns rs) tm
-| match_callstate:
-    forall f args targs k m tm cs tf
-           (TF: transl_fundef f = OK tf)
-           (MS: match_stacks j k cs)
-        (*(LD: Val.lessdef_list args targs)*)
-        (AINJ: val_list_inject j args targs)
-        (*(MEXT: Mem.extends m tm)*)
-        (MINJ: Mem.inject j m tm),
-      match_states j (CMinSel_Callstate f args k) m
-                   (RTL_Callstate cs tf targs) tm
-| match_returnstate:
-    forall v tv k m tm cs
-           (MS: match_stacks j k cs)
-        (*(LD: Val.lessdef v tv)*)
-        (VINJ: val_inject j v tv)
-        (*(MEXT: Mem.extends m tm)*)
-        (MINJ: Mem.inject j m tm),
-      match_states j (CMinSel_Returnstate v k) m
-                   (RTL_Returnstate cs tv) tm.
-
-
-
-Definition MATCH (d:RTL_core) mu c1 m1 c2 m2:Prop :=
-  match_states (restrict (as_inj mu) (vis mu)) c1 m1 c2 m2 /\
-  REACH_closed m1 (vis mu) /\
-  meminj_preserves_globals ge (as_inj mu) /\
-  globalfunction_ptr_inject (as_inj mu) /\
-  (forall b, isGlobalBlock ge b = true -> frgnBlocksSrc mu b = true) /\
-  sm_valid mu m1 m2 /\ SM_wd mu /\ Mem.inject (as_inj mu) m1 m2.
-
-Print effstep.
-Print rtl_eff_sem.
-Print vis.
-Print locBlocksSrc.
-
-Variable tprog: RTL.program.
-Let tge : RTL.genv := Genv.globalenv tprog.
-Print genv.
-
-Lemma MATCH_effcore_diagram: forall 
-                               st1 m1 st1' m1' (U1 : block -> Z -> bool) ge'
-                               (CS: effstep rtl_eff_sem ge' U1 st1 m1 st1' m1') (* unpacks the effect step. RTL_effstep. *)
-                               st2 mu m2 
-                               (UHyp: forall b z, U1 b z = true -> 
-                                                  Mem.valid_block m1 b -> vis mu b = true) (* Proof that allocated valid blocks are visible in the source*)
-                             (*(MTCH: MATCH st1 mu st1 m1 st2 m2)*),
-                             exists st2' m2' mu', exists U2 : block -> Z -> bool,
-                                                    (effstep_plus rtl_eff_sem tge U2 st2 m2 st2' m2' \/
-                                                     effstep_star rtl_eff_sem tge U2 st2 m2 st2' m2' (*/\ lt_state st1' st1*))
-                                                    /\ intern_incr mu mu' /\
-                                                    sm_inject_separated mu mu' m1 m2 /\
-                                                    sm_locally_allocated mu mu' m1 m2 m1' m2' /\
-                                                    (*MATCH st1' mu' st1' m1' st2' m2' /\ *)
-                                                    (forall (b : block) (ofs : Z),
-                                                       U2 b ofs = true ->
-                                                       Mem.valid_block m2 b /\
-                                                       (locBlocksTgt mu b = false ->
-                                                        exists (b1 : block) (delta1 : Z),
-                                                          foreign_of mu b1 = Some (b, delta1) /\
-                                                          U1 b1 (ofs - delta1)%Z = true /\
-                                                          Mem.perm m1 b1 (ofs - delta1) Max Nonempty)).
-  (*New script*)
-  intros st1 m1 st1' m1' U1 ge' CS. intros. 
-  eexists. exists m2, mu, EmptyEffect.
-  split.
-  right.
-
-
-
-
-
-
-  intros st1 m1 st1' m1' U1 ge'. CS.
-
-  induction CS; intros; eexists. (*12 Cases*)
-
-  (*Case: skip seq*)
-  exists m2, mu. 
-  exists EmptyEffect.
-  split.
-  right.
-  unfold vis in UHyp.
-  unfold effstep_star; exists O; simpl.
-  reflexivity.
-
-  split. 
-  apply intern_incr_refl.
-
-  split.
-  apply sm_inject_separated_same_sminj.
-
-  split.
-  Lemma sm_locally_allocated_refl: forall mu m1 m2, sm_locally_allocated mu mu m1 m2 m1 m2.
+    eapply match_regular_states; eauto.
+    apply match_stacks_inside_set_reg; auto.
+    apply agree_set_reg; auto.
+    
+
+    (* Istore *)
+    exploit tr_funbody_inv; eauto. intros TR; inv TR.
+    exploit eval_addressing_inject.
+    About eval_addressing_inject.
+    eapply match_stacks_inside_globals; eauto.
+    eexact SP.
+    instantiate (2 := rs##args). instantiate (1 := rs'##(sregs ctx args)). eapply agree_val_regs; eauto.
+    eauto.
+    fold saddr. intros [a' [P Q]].
+    exploit Mem.storev_mapped_inject; eauto. eapply agree_val_reg; eauto. 
+    intros [m2' [U V]].
+    assert (eval_addressing tge (Vptr sp' Int.zero) (saddr ctx addr) rs' ## (sregs ctx args) = Some a').
+    rewrite <- P. apply eval_addressing_preserved. exact symbols_preserved.
+    eexists. eexists.
+    split; simpl.
+    left.
+    eapply corestep_plus_one. eapply rtl_corestep_exec_Istore; eauto.
+
+    exists mu.
+    intuition.
+    apply intern_incr_refl.
+    apply sm_inject_separated_same_sminj.
+    loc_alloc_solve.
+
+
+    Focus.
+    destruct a; simpl in H1; try discriminate.
+    destruct a'; simpl in U; try discriminate.
+    unfold MATCH;
+    intuition.
+    econstructor; eauto.
+    eapply match_stacks_inside_store; eauto.
+    eapply Mem.store_valid_block_1; eauto.
+    eapply range_private_invariant; eauto.
+    intros; split; auto. eapply Mem.perm_store_2; eauto.
+    intros; eapply Mem.perm_store_1; eauto.
+    intros. eapply SSZ2. eapply Mem.perm_store_2; eauto.
+    inv H2.
+    eapply REACH_Store; 
+    try eassumption.
+    assert (VINJ1: val_inject (restrict (as_inj mu) (vis mu)) (Vptr b i) (Vptr b0 i0)).
+    admit.
+    inv VINJ1.
+    apply (restrictD_Some _ _ _ _ _ H15).
+     intros b' Hb'. rewrite getBlocksD, getBlocksD_nil in Hb'.
+     destruct (rs # src); inv Hb'. 
+     rewrite orb_false_r in H10.
+       rewrite H10. simpl.
+       assert (b1=b').
+       remember (eq_block b1 b') as d.
+          destruct d; intuition.
+       subst. 
+    assert (VINJ2: val_inject (restrict (as_inj mu) (vis mu)) (Vptr b' i) (Vptr b0 i0)).
+    admit.
+       inv VINJ2. apply (restrictD_Some _ _ _ _ _ H16).
+      (* sm_valid mu m1' m2' *)
+    split; intros. 
+      eapply storev_valid_block_1; try eassumption.
+      eapply H8; assumption.
+      eapply Mem.store_valid_block_1; try eassumption.
+      eapply H8; assumption.
+    
+
+
+(**)
+    (* Icall *)
+    Focus 1.
+    exploit match_stacks_inside_globalenvs; eauto. intros [bound G].
+    exploit find_function_agree; eauto. intros [fd' [A B]].
+    exploit tr_funbody_inv; eauto. intros TR. inv TR.
+
+    (* not inlined *)
+    eexists. eexists.
+    split; simpl.
+    left.
+    eapply corestep_plus_one. eapply rtl_corestep_exec_Icall; eauto.
+    Print rtl_corestep_exec_Icall.
+    eapply sig_function_translated; eauto.
+    exists mu.
+    intuition.
+    apply intern_incr_refl.
+    apply sm_inject_separated_same_sminj.
+    loc_alloc_solve.
+
+    unfold MATCH.
+    split.
+    econstructor; eauto.
+    eapply match_stacks_cons; eauto.
+    eapply agree_val_regs; eauto.   
+    intuition.
+
+    (* inlined *)
+    assert (fd = Internal f0).
+    simpl in H1. destruct (Genv.find_symbol ge id) as [b|] eqn:?; try discriminate.
+    exploit (funenv_program_compat SrcProg). 
+    try eassumption. eauto. intros. 
+    unfold ge in H1. congruence.
+    subst fd.
+    
+    eexists. eexists.
+    split; simpl.
+    right; split. simpl; omega.
+    eapply corestep_star_zero.
+
+    exists mu.
+    intuition.
+    apply intern_incr_refl.
+    apply sm_inject_separated_same_sminj.
+    loc_alloc_solve.
+
+    unfold MATCH;
+    intuition.
+    Focus 1.
+    eapply match_call_regular_states; eauto. (* match_call_regular_states*)
+    eapply match_stacks_inside_inlined; eauto.
+    red; intros. apply PRIV. inv H14. destruct H17.
+    xomega.
+    apply agree_val_regs_gen; auto.
+    red; intros; apply PRIV. destruct H17. omega.
+
+    (* Itailcall *)
+    exploit match_stacks_inside_globalenvs; eauto. intros [bound G].
+    exploit find_function_agree; eauto. intros [fd' [A B]].
+    assert (PRIV': range_private (as_inj mu) m1' m2 sp' (dstk ctx) f'.(fn_stacksize)).
+    eapply range_private_free_left; eauto. inv FB. rewrite <- H5. auto. 
+    exploit tr_funbody_inv; eauto. 
+    intros TR. 
+    inv TR.
+
+    (* within the original function *)
+    inv MS0; try congruence.
+
+    assert (X: { m1' | Mem.free m2 sp' 0 (fn_stacksize f') = Some m1'}).
+    apply Mem.range_perm_free. red; intros.
+    destruct (zlt ofs f.(fn_stacksize)). 
+    replace ofs with (ofs + dstk ctx) by omega. eapply Mem.perm_inject; eauto.
+    eapply Mem.free_range_perm; eauto. omega.
+    inv FB. eapply range_private_perms; eauto. xomega.
+    destruct X as [m2' FREE].
+    
+    eexists. eexists.
+    split; simpl.
+    left. 
+    eapply corestep_plus_one. eapply rtl_corestep_exec_Itailcall; eauto.
+    eapply sig_function_translated; eauto.
+    exists mu.
+    intuition.
+    apply intern_incr_refl.
+    apply sm_inject_separated_same_sminj.
+    loc_alloc_solve.
+     
+    
+    unfold MATCH.
+    intuition.
+    econstructor; eauto.
+    eapply match_stacks_bound with (bound := sp'). 
+    eapply match_stacks_invariant; eauto.
+    intros. eapply Mem.perm_free_3; eauto. 
+    intros. eapply Mem.perm_free_1; eauto. 
+    intros. eapply Mem.perm_free_3; eauto.
+    erewrite Mem.nextblock_free; eauto. red in VB; xomega.
+    eapply agree_val_regs; eauto.
+    eapply Mem.free_right_inject; eauto. eapply Mem.free_left_inject; eauto.
+    (* show that no valid location points into the stack block being freed *)
+    intros. rewrite DSTK in PRIV'. exploit (PRIV' (ofs + delta)). omega. intros [P Q]. 
+    eelim Q; eauto. replace (ofs + delta - delta) with ofs by omega. 
+    apply Mem.perm_max with k. apply Mem.perm_implies with p; auto with mem.
+    eapply REACH_closed_free; eauto.
+      (* sm_valid mu m1' m2' *)
+    split; intros. 
+      eapply Mem.valid_block_free_1; try eassumption.
+      eapply H7; assumption.
+      eapply Mem.valid_block_free_1; try eassumption.
+      eapply H7; assumption.
+      (*  Mem.inject (as_inj mu) m1' m2' *)
+      eapply Mem.free_right_inject; eauto. eapply Mem.free_left_inject; eauto.
+      (* show that no valid location points into the stack block being freed *)
+      intros. rewrite DSTK in PRIV'. exploit (PRIV' (ofs + delta)). omega. intros [P Q]. 
+      eelim Q; eauto. replace (ofs + delta - delta) with ofs by omega. 
+      apply Mem.perm_max with k. apply Mem.perm_implies with p; auto with mem.
+
+    (* turned into a call *)
+    eexists. eexists. split; simpl.
+    left. 
+    eapply corestep_plus_one. eapply rtl_corestep_exec_Icall; eauto.
+    eapply sig_function_translated; eauto.
+    
+    exists mu.
+    intuition.
+    apply intern_incr_refl.
+    apply sm_inject_separated_same_sminj.
+    loc_alloc_solve.
+
+    unfold MATCH.
+    intuition.
+    econstructor; eauto.
+    eapply match_stacks_untailcall; eauto.
+    eapply match_stacks_inside_invariant; eauto. 
+    intros. eapply Mem.perm_free_3; eauto.
+    eapply agree_val_regs; eauto.
+    eapply Mem.free_left_inject; eauto.
+    eapply REACH_closed_free; eauto.
+    
+    (*  sm_valid mu m1' m2 *)
+    split; intros. 
+      eapply Mem.valid_block_free_1; try eassumption.
+      eapply H7; assumption.
+      eapply H7; assumption.
+      (*  Mem.inject (as_inj mu) m1' m2' *)
+      eapply Mem.free_left_inject; eauto.
+
+    (* inlined *)
+    assert (fd = Internal f0).
+    simpl in H1. destruct (Genv.find_symbol ge id) as [b|] eqn:?; try discriminate.
+    exploit (funenv_program_compat SrcProg); eauto. intros. 
+    unfold ge in H1. congruence.
+    subst fd.
+    eexists. eexists.
+    split; simpl.
+    right; split. simpl; omega. 
+    eapply corestep_star_zero.
+
+    exists mu.
+    intuition.
+    apply intern_incr_refl.
+    apply sm_inject_separated_same_sminj.
+    loc_alloc_solve.
+
+    unfold MATCH;
+    intuition.
+    econstructor; eauto.
+    eapply match_stacks_inside_inlined_tailcall; eauto.
+    eapply match_stacks_inside_invariant; eauto.
+    intros. eapply Mem.perm_free_3; eauto.
+    apply agree_val_regs_gen; auto.
+    eapply Mem.free_left_inject; eauto.
+    red; intros; apply PRIV'. 
+    assert (dstk ctx <= dstk ctx'). red in H15; rewrite H15. apply align_le. apply min_alignment_pos.
+    omega.
+    eapply REACH_closed_free; eauto.
+    (* sm_valid mu m1' m2 *)
+    split; intros.
+      eapply Mem.valid_block_free_1; try eassumption.
+      eapply H11; assumption.
+      eapply H11; assumption.
+      (*  Mem.inject (as_inj mu) m1' m2' *)
+      eapply Mem.free_left_inject; eauto.
+
+
+    (* Icond *)
+
+    exploit tr_funbody_inv; eauto. intros TR; inv TR.
+    assert (eval_condition cond rs'##(sregs ctx args) m2 = Some b).
+    eapply eval_condition_inject; eauto. eapply agree_val_regs; eauto. 
+    
+    eexists. eexists. 
+    split; simpl.
+    left. 
+    eapply corestep_plus_one.
+    eapply rtl_corestep_exec_Icond; eauto.
+
+    exists mu. intuition.
+    apply intern_incr_refl.
+    apply sm_inject_separated_same_sminj.
+    loc_alloc_solve.
+
+    unfold MATCH.
+    intuition.
+    destruct b;
+      econstructor; eauto.
+
+
+    (* jumptable *)
+    exploit tr_funbody_inv; eauto. intros TR; inv TR.
+    assert (val_inject (as_inj mu) rs#arg rs'#(sreg ctx arg)). eapply agree_val_reg; eauto.
+    rewrite H1 in H3; inv H3.
+    
+    eexists. eexists.
+    split; simpl.
+    left.
+    eapply corestep_plus_one. eapply rtl_corestep_exec_Ijumptable; eauto.
+    rewrite list_nth_z_map. rewrite H2. simpl; reflexivity. 
+    
+    exists mu. intuition.
+    apply intern_incr_refl.
+    apply sm_inject_separated_same_sminj.
+    loc_alloc_solve.
+
+    unfold MATCH.
+    intuition.
+    econstructor; eauto.
+
+    (* return *)
+    exploit tr_funbody_inv; eauto. intros TR; inv TR.
+
+    (* not inlined *)
+    inv MS0; try congruence.
+    assert (X: { m1' | Mem.free m2 sp' 0 (fn_stacksize f') = Some m1'}).
+    apply Mem.range_perm_free. red; intros.
+    destruct (zlt ofs f.(fn_stacksize)). 
+    replace ofs with (ofs + dstk ctx) by omega. eapply Mem.perm_inject; eauto.
+    eapply Mem.free_range_perm; eauto. omega.
+    inv FB. eapply range_private_perms; eauto.
+    generalize (Zmax_spec (fn_stacksize f) 0). destruct (zlt 0 (fn_stacksize f)); omega.
+    destruct X as [m2' FREE].
+    
+    eexists. eexists.
+    split; simpl.
+    left.
+    eapply corestep_plus_one. eapply rtl_corestep_exec_Ireturn; eauto. 
+    
+    exists mu.
+    intuition.
+    apply intern_incr_refl.
+    apply sm_inject_separated_same_sminj.
+    loc_alloc_solve.
+
+    unfold MATCH;
+    intuition.
+    econstructor; eauto.
+    eapply match_stacks_bound with (bound := sp'). 
+    eapply match_stacks_invariant; eauto.
+    intros. eapply Mem.perm_free_3; eauto. 
+    intros. eapply Mem.perm_free_1; eauto. 
+    intros. eapply Mem.perm_free_3; eauto.
+    erewrite Mem.nextblock_free; eauto. red in VB; xomega.
+    destruct or; simpl. apply agree_val_reg; auto. auto.
+
+    eapply Mem.free_right_inject; eauto. eapply Mem.free_left_inject; eauto.
+    (* show that no valid location points into the stack block being freed *)
+    intros. inversion FB; subst.
+    assert (PRIV': range_private (as_inj mu) m1' m2 sp' (dstk ctx) f'.(fn_stacksize)).
+    rewrite H16 in PRIV. eapply range_private_free_left; eauto. 
+    rewrite DSTK in PRIV'. exploit (PRIV' (ofs + delta)). omega. intros [A B]. 
+    eelim B; eauto. replace (ofs + delta - delta) with ofs by omega. 
+    apply Mem.perm_max with k. apply Mem.perm_implies with p; auto with mem.
+
+    eapply REACH_closed_free; eauto.
+
+    (*  sm_valid mu m1' m2 *)
+    split; intros.
+      eapply Mem.valid_block_free_1; try eassumption.
+      eapply H8; assumption.
+      eapply Mem.valid_block_free_1; try eassumption.
+      eapply H8; assumption.
+      (*  Mem.inject (as_inj mu) m1' m2' *)
+ eapply Mem.free_right_inject; eauto. eapply Mem.free_left_inject; eauto.
+    (* show that no valid location points into the stack block being freed *)
+    intros. inversion FB; subst.
+    assert (PRIV': range_private (as_inj mu) m1' m2 sp' (dstk ctx) f'.(fn_stacksize)).
+    rewrite H16 in PRIV. eapply range_private_free_left; eauto. 
+    rewrite DSTK in PRIV'. exploit (PRIV' (ofs + delta)). omega. intros [A B]. 
+    eelim B; eauto. replace (ofs + delta - delta) with ofs by omega. 
+    apply Mem.perm_max with k. apply Mem.perm_implies with p; auto with mem.
+
+
+    (* inlined *)
+    eexists. eexists.             
+    split; simpl.
+    right; split; simpl. omega.
+    
+    eapply corestep_star_zero.
+
+    exists mu.
+    intuition.
+    apply intern_incr_refl.
+    apply sm_inject_separated_same_sminj.
+    loc_alloc_solve. 
+    
+    unfold MATCH;
+    intuition.
+    econstructor; eauto.
+    
+    
+  eapply match_stacks_inside_invariant; eauto. 
+    intros. eapply Mem.perm_free_3; eauto.
+  destruct or; simpl. apply agree_val_reg; auto. auto.
+  eapply Mem.free_left_inject; eauto.
+  inv FB. subst.  rewrite H13 in PRIV. eapply range_private_free_left; eauto.
+  
+    eapply REACH_closed_free; eauto.
+    (*sm_valid*)
+    split; intros.
+      eapply Mem.valid_block_free_1; try eassumption.
+      eapply H8; assumption.
+      eapply H8; assumption.
+      (*  Mem.inject (as_inj mu) m1' m2 *)
+      eapply Mem.free_left_inject; eauto.
+
+    (* internal function, not inlined *)
+    assert (A: exists f', tr_function fenv f f' /\ fd' = Internal f'). 
+    Errors.monadInv FD. exists x. split; auto. eapply transf_function_spec; eauto. 
+    destruct A as [f' [TR EQ]]. inversion TR; subst.
+    repeat open_Hyp.
+    exploit alloc_parallel_intern; 
+    eauto. apply Zle_refl. 
+    instantiate (1 := fn_stacksize f'). inv H1. xomega.
+    intros [mu' [m2' [sp' [A [B [C [D E]]]]]]].
+    
+    eexists. eexists.
+    split; simpl.
+    left.
+    eapply corestep_plus_one. eapply rtl_corestep_exec_function_internal; eauto.
+
+    rewrite H5.
+    exists mu'. 
+    intuition.
+
+    unfold MATCH; intuition.
+    rewrite H6.
+    rewrite <- H5.
+    eapply match_regular_states.
+    apply match_stacks_inside_base.
+  assert (SP: sp' = Mem.nextblock m2) by (eapply Mem.alloc_result; eauto).
+  rewrite <- SP in MS0. 
+  eapply (match_stacks_invariant mu); eauto.
+    eapply intern_incr_as_inj; eauto.
+    intros. destruct (eq_block b1 stk). 
+    subst b1. rewrite D in H20; inv H20. subst b2. eelim Plt_strict; eauto.  
+    rewrite H14 in H20; auto. 
+    intros. exploit Mem.perm_alloc_inv. eexact H0. eauto. 
+    destruct (eq_block b1 stk); intros; auto. 
+    subst b1. rewrite D in H20; inv H20. subst b2. eelim Plt_strict; eauto.  
+    intros. eapply Mem.perm_alloc_1; eauto. 
+    intros. exploit Mem.perm_alloc_inv. eexact A. eauto. 
+    rewrite dec_eq_false; auto.
+  auto. auto. auto. 
+  rewrite H5. apply agree_regs_init_regs.
+  eapply val_list_inject_incr.
+  Lemma inject_incr_structure: forall mu mu' (II: intern_incr mu mu'), inject_incr (as_inj mu) (as_inj mu').
   Admitted.
-  apply sm_locally_allocated_refl.
-  intros. unfold EmptyEffect in H0.
-  contradict H0; auto.
+  eapply inject_incr_structure; eauto.
+  eauto.
+  auto. inv H1; auto. congruence. auto.
+  eapply Mem.valid_new_block; eauto.
+  red; intros. split.
+  eapply Mem.perm_alloc_2; eauto. inv H1; xomega.
+  intros; red; intros. exploit Mem.perm_alloc_inv. eexact H0. eauto.
+  destruct (eq_block b stk); intros. 
+  subst. rewrite D in H21; inv H21. inv H1; xomega.
+  rewrite H14 in H21; auto. eelim Mem.fresh_block_alloc. eexact A. eapply Mem.mi_mappedblocks; eauto.
+  auto.
+  intros. exploit Mem.perm_alloc_inv; eauto. rewrite dec_eq_true. omega.
 
-  (*Case: skip block*)
-  exists m2, mu.
-  exists EmptyEffect. (*This should change*)
-  split. 
-  right.
-  unfold effstep_star; exists O; simpl.
-  reflexivity.
-
-  split.
-  apply intern_incr_refl.
-
-  split.
-  apply sm_inject_separated_same_sminj.
-
-  split.
-  apply sm_locally_allocated_refl.
-
-  intros. unfold EmptyEffect in H1.
-  contradict H1; auto.
-
-  (*Case: skip return*)
-  exists m2, mu.
-  exists EmptyEffect. (*This should change*)
-  split. 
-  right.
-  unfold effstep_star; exists O; simpl.
-  reflexivity.
-
-  split.
-  apply intern_incr_refl.
-
-  split.
-  apply sm_inject_separated_same_sminj.
-
-  split.
-  apply sm_locally_allocated_refl.
-
-  intros. unfold EmptyEffect in H2.
-  contradict H2; auto.
-
-  (*assign*)
-
-  exists m2, mu.
-
-  exists EmptyEffect. (*This should change*)
-  split. 
-  right.
-  unfold effstep_star. exists O. simpl.
-  reflexivity.
-
-  split.
-  apply intern_incr_refl.
-
-  split.
-  apply sm_inject_separated_same_sminj.
+  (* meminj_preserves_globals ge (as_inj mu') 
+  unfold meminj_preserves_globals in H9.
+   destruct H9 as [A' [B' C']].
+   unfold meminj_preserves_globals; intros. 
+   repeat split; intros.
+   destruct (eq_block b stk); intros. 
+   subst b. 
+   rewrite D.*)
+   
+  admit.
+  admit.
 
 
-  split. admit.
+    (* internal function, inlined *)
+    inversion FB; subst.
+    exploit Mem.alloc_left_mapped_inject. 
+    eauto.
+    eauto.
+    (* sp' is valid *)
+    instantiate (1 := sp'). auto.
+    (* offset is representable *)
+    instantiate (1 := dstk ctx). generalize (Zmax2 (fn_stacksize f) 0). omega.
+    (* size of target block is representable *)
+    intros. right. exploit SSZ2; eauto with mem. inv FB; omega.
+    (* we have full permissions on sp' at and above dstk ctx *)
+    intros. apply Mem.perm_cur. apply Mem.perm_implies with Freeable; auto with mem.
+    eapply range_private_perms; eauto. xomega.
+    (* offset is aligned *)
+    replace (fn_stacksize f - 0) with (fn_stacksize f) by omega.
+    inv FB. apply min_alignment_sound; auto.
+    (* nobody maps to (sp, dstk ctx...) *)
+    intros. exploit (PRIV (ofs + delta')); eauto. xomega.
+    intros [A B]. eelim B; eauto.
+    replace (ofs + delta' - delta') with ofs by omega.
+    apply Mem.perm_max with k. apply Mem.perm_implies with p; auto with mem.
+    intros [F' [A [B [C D]]]].
+    exploit tr_moves_init_regs; eauto. intros [rs'' [P [Q R]]].
+    eexists. eexists.
+    split; simpl. 
+    left.
+    eapply corestep_plus_one. eapply rtl_corestep_exec_Inop; eauto. 
+    Print star.
+    (* eexact P. traceEq.
+  eapply match_regular_states.
+  econstructor.
+  eapply match_stacks_inside_alloc_left; eauto.
+  eapply match_stacks_inside_invariant; eauto.
+  omega.
+  auto.
+  apply agree_regs_incr with F; auto.
+  auto. auto. auto.
+  rewrite H2. eapply range_private_alloc_left; eauto.
+  auto. auto.*)
+    clear P. admit.
+    
 
-  intros. unfold EmptyEffect in H2.
-  contradict H2; auto.
+    (* external function *)
+    (*  exploit match_stacks_globalenvs; eauto. intros [bound MG].
+  (*exploit external_call_mem_inject; eauto.
+    eapply match_globalenvs_preserves_globals; eauto.
+    Check external_call.
+    Print extcall_sem. 
+  intros [F1 [v1 [m1' [A [B [C [D [E [J K]]]]]]]]].*)
+  simpl in FD. inv FD. 
+  left; econstructor; split.
+  eapply plus_one. eapply exec_function_external; eauto. 
+    eapply external_call_symbols_preserved; eauto. 
+    exact symbols_preserved. exact varinfo_preserved.
+  econstructor.
+    eapply match_stacks_bound with (Mem.nextblock m'0).
+    eapply match_stacks_extcall with (F1 := F) (F2 := F1) (m1 := m) (m1' := m'0); eauto.
+    intros; eapply external_call_max_perm; eauto. 
+    intros; eapply external_call_max_perm; eauto.
+    xomega.
+    eapply external_call_nextblock; eauto. 
+    auto. auto.*)
 
+    (* return fron noninlined function *)
+    inv MS0.
+    (* normal case *)
+    eexists. eexists.
+    split; simpl.
+    left.
+    eapply corestep_plus_one. eapply rtl_corestep_exec_return.
+    
+    exists mu. intuition.
+    apply intern_incr_refl.
+    apply sm_inject_separated_same_sminj.
+    loc_alloc_solve.
 
+    unfold MATCH; intuition.
+    econstructor; eauto. 
+    apply match_stacks_inside_set_reg; auto. 
+    apply agree_set_reg; auto.
+    
+    (* untailcall case *)
+    inv MS; try congruence.
+    rewrite RET in RET0; inv RET0.
+    (*
+  assert (rpc = pc). unfold spc in H0; unfold node in *; xomega.
+  assert (res0 = res). unfold sreg in H1; unfold reg in *; xomega.
+  subst rpc res0.
+     *)
+    eexists. eexists.     
+    split; simpl.
+    left.
+    eapply corestep_plus_one. eapply rtl_corestep_exec_return.
+    exists mu. intuition.
+    apply intern_incr_refl.
+    apply sm_inject_separated_same_sminj.
+    loc_alloc_solve.
 
+    unfold MATCH. intuition.
+    eapply match_regular_states. 
+    eapply match_stacks_inside_set_reg; eauto.
+    auto. 
+    apply agree_set_reg; auto.
+    auto. auto. auto.
+    red; intros. destruct (zlt ofs (dstk ctx)). apply PAD; omega. apply PRIV; omega.
+    auto. auto. 
+    
+    (* return from inlined function *)
+    inv MS0; try congruence. rewrite RET0 in RET; inv RET. 
+    unfold inline_return in AT. 
+    assert (PRIV': range_private (as_inj mu) m1' m2 sp' (dstk ctx' + mstk ctx') f'.(fn_stacksize)).
+    red; intros. destruct (zlt ofs (dstk ctx)). apply PAD. omega. apply PRIV. omega.
+    (* with a result *)
+    destruct or.
+    eexists. eexists.
+    split; simpl.
+    left. 
+    eapply corestep_plus_one.
+    eapply rtl_corestep_exec_Iop; eauto. simpl. reflexivity.
+    
+    exists mu. intuition.
+    apply intern_incr_refl.
+    apply sm_inject_separated_same_sminj.
+    loc_alloc_solve.
 
-  split_allsplit.
-
-  eexists.
-  eexists.
-  eexists.
-  eexists.
-  eexists.
-  split. (* effste*)
-  unfold effstep_plus.
-  unfold effstep_star.
-  (*Lemma about effstepN.*)
-
-  Focus 2. split.
-  (*intern_incr
-unfold intern_incr.*)
-
-  Focus 2. split.
-  unfold sm_inject_separated.
-
-  Focus 2. split.
-  unfold sm_locally_allocated.
+    unfold MATCH; intuition.
+    econstructor; eauto. apply match_stacks_inside_set_reg; auto. apply agree_set_reg; auto.
+    (* without a result *)
+    eexists. eexists.
+    split; simpl. left.  
+    eapply corestep_plus_one. eapply rtl_corestep_exec_Inop; eauto.
+    exists mu. intuition.
+    apply intern_incr_refl.
+    apply sm_inject_separated_same_sminj.
+    apply sm_locally_allocatedChar.
+    repeat split; extensionality b0;
+    rewrite freshloc_irrefl;
+    intuition.
+    unfold MATCH; intuition.
+    econstructor; eauto. subst vres. apply agree_set_reg_undef'; auto.
+  Qed.
